More comments, references

src/fol.lean
@@ -1,6 +1,49 @@
 import data.set
 import tactic.linarith
 
+/-!
+# First-order predicate logic
+
+In this file we define the syntax of intuitionistic first-order logic and a natural deduction
+proof calculus. 
+
+## Main result
+
+- `formula 𝒮` : the definition of first-order formulas over a signature 𝒮
+- `proof 𝒮`   : the definition of proof terms of natural deduction over a signature 𝒮
+
+## Notations
+
+We define the following notations for lifts and substitutions:
+
+- `X ↑ m ＠ i` for `lift X s k`  where `X` can be a term, a formula or a set of formulas.
+- `X[ s ⁄ k ]` for `subst X s k` where `X` can be a term, a formula or a set of formulas.
+- `Γ ⊢ φ` for proof Γ φ  
+
+We use the following local notations
+
+- `::` for `set.insert`
+
+## Notes
+
+We wrote comments whenever we felt like a topic wasn't really covered by the literature referenced.
+This includes some definitions that are not part of the actual implementation but simplify talking about it.
+
+## References
+
+* [N.G. de Bruijn, *Lambda calculus notation with nameless dummies*] [DB72]
+  -- the original paper describing what is now called de Bruijn indices
+* [J.M. Han, F.van Doorn, *A Formal Proof of the Independence of the Continuum Hypothesis*] [HvD20]
+  -- which we followed in their implementation of first-order logic using "partially applied" terms and formulas 
+  -- See also: https://flypitch.github.io/
+* [M.Huth, M. Ryan, *Logic in computer science*] [HR04]
+  -- for their development of the natural deduction proof calculus
+* [S. Berghofer, C. Urban, *A Head-to-Head Comparison of de Bruijn Indices and Names*] [BH07]
+  -- for a good breakdown of the proof of the substitution lemma `subst_subst`
+* https://github.com/coq-community/dblib/blob/master/src/DeBruijn.v 
+  -- as a good reference on lifting and substitution lemmas for de Bruijn indices
+-/
+
 -- use with `simp only with tls`
 mk_simp_attribute tls
 "Collection of definitions and lemmas for simplifying combinations of lifts and substitutions we would consider trivial."
@@ -8,45 +51,97 @@ mk_simp_attribute tls
 open nat set
 namespace fol
 universe variable u
+
+/-- A signature of a first-order logic defining its function and predicate symbols with arities. -/
+structure signature : Type (u+1) :=
+(func_symb : ℕ → Type u) (pred_symb : ℕ → Type u)
+
+def signature.constants (𝒮 : signature) := 𝒮.func_symb 0
+
+inductive sorry_nothing : ℕ → Type u
+
+def trivial_signature : signature :=
+{ func_symb := sorry_nothing, pred_symb := sorry_nothing}
+
+
+/-! ### terms -/
+variable (𝒮 : signature.{u})
+
 /--
-  The language of a first-order logic consisting of functions and predicates with given arities.
--/
-structure language : Type (u+1) :=
-(functions : ℕ → Type u) ( predicates : ℕ → Type u)
-
-inductive empty : ℕ → Type
-
-def trivial_lang : language :=
-{ functions := empty, predicates := empty}
-
-variable (L : language.{u})
- 
-/--
-  `preterm L a` is partially applied* first-order term of `L`, representing variabes as De Bruijn indices.
-
-  * For `a=0` this is a well-formed term.
-  * For `a≠0` this is a partially applied function, requiring `a` further term applications to become
-    a well formed term.
+  `preterm 𝒮 a` is partially applied term of first-order logic over the signature `𝒮`.
+  If applied to `a` terms it becomes a well-formed term.
 -/
 inductive preterm : ℕ → Type u
-| var  ( index : ℕ ) : preterm 0
-| func { arity : ℕ } ( f : L.functions arity ) : preterm arity
-| fapp { arity : ℕ } ( t : preterm (arity+1) )  ( s : preterm 0 ) : preterm arity
+| var  (index : ℕ) : preterm 0
+| func {arity : ℕ} (f : 𝒮.func_symb arity) : preterm arity
+| fapp {arity : ℕ} (t : preterm (arity+1))  (s : preterm 0) : preterm arity
+
 export preterm
 
-@[reducible] def term := preterm L 0
 prefix `#`:max := preterm.var
+@[reducible] def term := preterm 𝒮 0
 
-variable {L}
+variable {𝒮}
+
+/-  
+  ## Definition - variables at `k`  
+  
+  Let `t` be a term. The variables of `t` are defined by structural induction in the obvious way.
+
+  Let `k ∈ ℕ`. The variables of `t` *at reference depth `k`* or simply *at `k`* are the variables 
+  of `t` such that their index is equal to `k`. 
+
+  A variable of `t` is called *`k`-free* if its index is greater than `k`.
+
+  The term `t` is called *`k`-free* if it all its variables are `k`-free.
+
+  ## Remark
+  The terminology of "reference depth" comes from de Bruijn's original paper. 
+  What do these variable indices reference? 
+  In the case of terms is easy to explain.
+  One should first imagine an sequence (called the environment) 
+      `...,x₃,x₂,x₁,x₀`
+  of what we will call "variable binders".
+
+  Variables at reference depth `k` then should be thought of referencing `xₖ`,
+  or, our preferred terminology, `xₖ` binds the variables at `k`.
+  The reason for writing this sequence from left to right will hopefully become apparent 
+  when we introduce formulas.
+
+  We will sometimes refer to variable binders as variables of the environment or simply variable
+  if it does not cause confusion.
+-/
+
+
 namespace term
+
+/-
+  Even though we technically have an infinite amount of variables
+  it is often very convenient to be able to add "fresh" variables
+  to the environment. In the most common case one adds a single new
+  variable right at the start of our imagined environment:
+    `...,x₃,x₂,x₁,x₀` to `...,x₃,x₂,x₁,x₀,y`. 
+  If we want the variables of `t` to reference the same variable binder
+  we will need to increase all indices by `1`. 
+  Doing so also ensures that the variable binder `y` is truly 
+  "fresh" for `t` in the sense that no variable of `t` is bound by it.
+
+  The case for adding `m` fresh variables at index `i` to the environment 
+  follows similarly.
+  It describes the change from
+    `...xᵢ₊₁,xᵢ,xᵢ₋₁,...,x₃,x₂,x₁,x₀`
+  to the new environment 
+    `....xᵢ₊₁,xᵢ,yₘ₋₁,...,y₀,xᵢ₋₁,...,x₃,x₂,x₁,x₀`.
+  We ensure consistent variable bindings of a term `t` by adding 
+  `m` to each `i`-free variable of `t`.
+
+  This operation on terms is know as a lift (or sometimes shift).
+-/
+
 /--
   `lift t m i` increases the index of each `i`-free variable in `t` by `m`.
-
-  * a variable is `i`-free if its De Bruijn index is greater than or equal to `i`.
-  * Notation:  `t ↑ m ＠ i`
-  * Note: We read this as "lift term `t` by `m` at `i`", which then informs the naming of later lemmas and our notation.
 -/
-def lift : ∀{a} , preterm L a → ℕ → ℕ → preterm L a 
+def lift : ∀{a} , preterm 𝒮 a → ℕ → ℕ → preterm 𝒮 a 
 | _ #x          m i := #( if i ≤ x then x+m else x)
 | _ (func f)    m i := func f
 | _ (fapp t s)   m i := fapp (lift t m i) (lift s m i)
@@ -54,43 +149,37 @@ def lift : ∀{a} , preterm L a → ℕ → ℕ → preterm L a
 end term
 
 notation t ` ↑ `:90 m ` ＠ `:90 i:90  := term.lift t m i
-notation t ` ↑₀ `:90 m :90 := term.lift t m 0
 
 namespace term
 
 -- unfolding lemmas for the simplifier
-@[simp, tls] lemma lift_fapp {a} (t : preterm L (a+1)) (s : preterm L 0) (m i : ℕ ) 
+@[simp, tls] lemma lift_fapp {a} (t : preterm 𝒮 (a+1)) (s : preterm 𝒮 0) (m i : ℕ) 
   : (fapp t s) ↑ m ＠ i = fapp (t ↑ m ＠ i) (s ↑ m ＠ i) := by refl
-@[simp, tls] lemma lift_func {a} (f : L.functions a) (m i : ℕ ) 
+@[simp, tls] lemma lift_func {a} (f : 𝒮.func_symb a) (m i : ℕ ) 
   : (func f) ↑ m ＠ i = func f := by refl
 
 -- lifting of variables by cases for the simplifier
-@[simp] lemma lift_var_lt {x m i : ℕ} (H : x < i) : #x ↑ m ＠ i = (#x : term L) 
+@[simp] lemma lift_var_lt {x m i : ℕ} (H : x < i) : #x ↑ m ＠ i = (#x : term 𝒮) 
   := begin unfold lift, rw if_neg (not_le.mpr H), end
-@[simp, tls] lemma lift_var_eq {x m}: ((#x ↑ m ＠ x) = (#(x+m) : term L)) 
+@[simp, tls] lemma lift_var_eq {x m}: ((#x ↑ m ＠ x) = (#(x+m) : term 𝒮)) 
   := begin rw lift, rw if_pos x.le_refl, end
-@[simp] lemma lift_var_gt {x m i} (H : i < x ) : #x ↑ m ＠ i = (#(x+m) : term L)
+@[simp] lemma lift_var_gt {x m i} (H : i < x ) : #x ↑ m ＠ i = (#(x+m) : term 𝒮)
   := begin rw lift, rw if_pos (le_of_lt H), end
-@[simp] lemma lift_var_ge {x m i} (H : i ≤ x ) : #x ↑ m ＠ i = (#(x+m) : term L)
+@[simp] lemma lift_var_ge {x m i} (H : i ≤ x ) : #x ↑ m ＠ i = (#(x+m) : term 𝒮)
   := begin rw lift, rw if_pos H, end
-@[simp] lemma lift_var_nge {x m i : ℕ} (H : ¬ i ≤ x) : #x ↑ m ＠ i = (#x : term L) 
+@[simp] lemma lift_var_nge {x m i : ℕ} (H : ¬ i ≤ x) : #x ↑ m ＠ i = (#x : term 𝒮) 
   := begin unfold lift, rw if_neg H, end
 
 
-/--
-  Lifting by `0` is trivial.
--/
-@[simp, tls] lemma lift_by_0: ∀ {a} ( t : preterm L a) {i}, t ↑ 0 ＠ i = t
+@[simp, tls] lemma lift_by_0: ∀ {a} ( t : preterm 𝒮 a) {i}, t ↑ 0 ＠ i = t
 | _ #x         i  := by simp[lift]
 | _ (func f)   _  := by refl
 | _ (fapp f t) _  := begin unfold lift, congr; apply lift_by_0, end
 
 
--- A collection of various lifting lemmas
--- collected through https://github.com/coq-community/dblib/blob/master/src/DeBruijn.v
--- and www21.in.tum.de/~berghofe/papers/LFMTP06.pdf
+/- Various lifting lemmas. -/
 
-lemma lift_lift: ∀ {a} ( t : preterm L a ) (m) {i} (n) {j} (H : j ≤ i), 
+lemma lift_lift: ∀ {a} ( t : preterm 𝒮 a ) (m) {i} (n) {j} (H : j ≤ i), 
   (t ↑ m ＠ i) ↑ n ＠ j = (t ↑ n ＠ j) ↑ m ＠ (i+n) 
 | _ #x          m i n j H   := 
   begin by_cases h₀ : i ≤ x,
@@ -105,7 +194,7 @@ lemma lift_lift: ∀ {a} ( t : preterm L a ) (m) {i} (n) {j} (H : j ≤ i),
 | _ (fapp f t)  _ _ _ _ _   := by simp*
     
 
-lemma lift_lift_rev {a} ( t : preterm L a ) {m i} (n) {j} (H : i + m ≤ j)
+lemma lift_lift_reverse {a} ( t : preterm 𝒮 a ) {m i} (n) {j} (H : i + m ≤ j)
     : (t ↑ m ＠ i) ↑ n ＠ j = ( t ↑ n ＠ (j-m) ) ↑  m  ＠ i :=
 begin
   have h : i ≤ (j-m) := nat.le_sub_right_of_add_le H,
@@ -113,7 +202,7 @@ begin
   rw [lift_lift t n m h, nat.sub_add_cancel h'],
 end
 
-lemma lift_lift_merge: ∀ {a} ( t : preterm L a) {m i} (n) {j} (H : i ≤ j) (H' : j ≤ i + m), 
+lemma lift_lift_merge: ∀ {a} ( t : preterm 𝒮 a) {m i} (n) {j} (H : i ≤ j) (H' : j ≤ i + m), 
   (t ↑ m ＠ i ) ↑ n ＠ j = t ↑ (m+n) ＠ i
 | _ #x         m i n j H H' :=  
   begin by_cases h₀ : i ≤ x,
@@ -125,51 +214,67 @@ lemma lift_lift_merge: ∀ {a} ( t : preterm L a) {m i} (n) {j} (H : i ≤ j) (H
 | _ (func f)   _ _ _ _ _ _  := by refl
 | _ (fapp t s) _ _ _ _ _ _  := by simp*
 
-lemma lift_by_succ {a} ( t : preterm L a) {m i} : t ↑ (m+1) ＠ i  = ( t ↑ 1 ＠ i) ↑ m ＠ i
+lemma lift_by_succ {a} ( t : preterm 𝒮 a) {m i} : t ↑ (m+1) ＠ i  = ( t ↑ 1 ＠ i) ↑ m ＠ i
   := begin rw[lift_lift_merge, one_add], apply le_refl, apply le_succ, end
 
+/-
+  Another common operation on the environment comes in the form of substitution.
+  For example, this is the case whenever we write "Let xₖ = s" in a proof.
+  Substituting `s` for `xₖ` in a term `t`, naively, should replace each
+  variable at `k` by `s`.
+  One obvious problem is that `s` could still be referencing `xₖ`.
+  We can avoid this by informally removing `xₖ` from the environment,
+  i.e. by decreasing each `k+1`-free variable during substitution by 1.
+  Another thing to consider is that the variables bound by `xₖ` 
+  are by definition `k`-free,  while this is not necessarily true for the term `s`. 
+
+  If we imagine our environment as a timeline objects we have defined or constructed,
+  then each `xₖ` should only depend on the objects `...,xₖ₊₂,xₖ₊₁` that came before.
+  Naive substitution however breaks the chronology of this timeline.
+
+  Thus, to ensure we replace a `k`-free term by another `k`-free term (and keep chronology), 
+  we define a form of capture-free substitution as below.
+-/
 
 /-- 
-  `subst t s k` subsitutes each occurences of `#k` in `t` for `s ↑ k ＠ 0` and 
-  reduces the index of all variables above `k` by `1`.
+  `subst t s k` substitutes `s ↑ k ＠ 0` for each variable at `k` in `t` and 
+  reduces the index of all `k+1`-free variables by `1`.
 -/
-def subst: ∀{a}, preterm L a → term L → ℕ → preterm L a
+def subst: ∀{a}, preterm 𝒮 a → term 𝒮 → ℕ → preterm 𝒮 a
 | _ #x           s k := if x < k then #x else if k < x then #(x-1) else (s ↑ k ＠ 0)
 | _ (func f)     s k := func f
 | _ (fapp t₁ t₂) s k := fapp (subst t₁ s k) (subst t₂ s k)
 
 end term
 
--- we use ⁄ (U+2044) instead of the usual slash / (U+002F) to avoid conflict with the divison operator
+-- we use ⁄ (U+2044) instead of the usual slash / (U+002F) to avoid conflict with the division operator
 -- recommended to make a custom shortcut as the default \textfractionsolidus is quite unhandy
 notation t `[`:max s ` ⁄ `:95 n `]`:0 := term.subst t s n 
-#reduce #5[#2 ⁄ 1]
+-- #reduce #5[#2 ⁄ 1]
 
 namespace term
 
 -- lemmas for the simplifier
-@[simp, tls] lemma subst_fapp {a} (t₁ : preterm L (a+1)) (t₂ s : preterm L 0) (k : ℕ ) : 
+@[simp, tls] lemma subst_fapp {a} (t₁ : preterm 𝒮 (a+1)) (t₂ s : preterm 𝒮 0) (k : ℕ ) : 
   (fapp t₁ t₂) [s ⁄ k] = fapp (t₁ [s ⁄ k]) (t₂ [s ⁄ k]) := by refl
-@[simp, tls] lemma subst_func {a} (f : L.functions a) (s k) : 
+@[simp, tls] lemma subst_func {a} (f : 𝒮.func_symb a) (s k) : 
   (func f) [s ⁄ k] = func f := by refl
 
-
-@[simp] lemma subst_var_lt (s : term L) {x k : ℕ} (H : x < k) : #x[s ⁄ k] = #x := 
+@[simp] lemma subst_var_lt (s : term 𝒮) {x k : ℕ} (H : x < k) : #x[s ⁄ k] = #x := 
     begin rw subst, rw if_pos H, end
-@[simp, tls] lemma subst_var_eq (s : term L) {k : ℕ}  : #k[s ⁄ k] =  s ↑ k ＠ 0 := 
+@[simp, tls] lemma subst_var_eq (s : term 𝒮) {k : ℕ}  : #k[s ⁄ k] =  s ↑ k ＠ 0 := 
     begin rw subst, repeat{ rw if_neg (lt_irrefl k) }, end
-@[simp] lemma subst_var_gt (s : term L) {x k  : ℕ} (H : k < x) : #x[s ⁄ k] = #(x-1) := 
+@[simp] lemma subst_var_gt (s : term 𝒮) {x k  : ℕ} (H : k < x) : #x[s ⁄ k] = #(x-1) := 
     begin rw subst, rw if_neg (lt_asymm H), rw if_pos H, end
-@[simp] lemma subst_var_nle (s : term L) {x k : ℕ} (H : ¬ (x ≤ k)) : #x[s ⁄ k] = #(x-1) := 
+@[simp] lemma subst_var_nle (s : term 𝒮) {x k : ℕ} (H : ¬ (x ≤ k)) : #x[s ⁄ k] = #(x-1) := 
   subst_var_gt s (not_le.mp H)
 
-@[simp, tls] lemma subst_var0 (s : term L): #0[ s ⁄ 0 ] = s := 
+@[simp, tls] lemma subst_var0 (s : term 𝒮): #0[ s ⁄ 0 ] = s := 
     begin rw subst_var_eq, exact lift_by_0 s, end
 
 
 -- substitution lemmas
-
-lemma lift_subst : ∀ {a}  (t : preterm L a) (s: term L) (m) {i} (k) ( H: i ≤ k ),
+lemma lift_subst : ∀ {a}  (t : preterm 𝒮 a) (s: term 𝒮) (m) {i} (k) ( H: i ≤ k ),
     t [ s ⁄ k ] ↑ m ＠ i = (t ↑ m ＠ i )[ s ⁄ k+m ] 
 | _ #x s m i k H := 
   begin 
@@ -192,7 +297,7 @@ lemma lift_subst : ∀ {a}  (t : preterm L a) (s: term L) (m) {i} (k) ( H: i ≤
 | _ (func f)   _ _ _ _ _ := by refl
 | _ (fapp f t) _ _ _ _ _ := by simp* 
 
-lemma subst_lift: ∀  {a}  (t : preterm L a) (s: term L) {m i k : ℕ} (H: i ≤ k) (H' : k ≤ i + m),
+lemma subst_lift: ∀  {a}  (t : preterm 𝒮 a) (s: term 𝒮) {m i k : ℕ} (H: i ≤ k) (H' : k ≤ i + m),
     (t ↑ (m+1) ＠ i) [s ⁄ k] = t ↑ m ＠ i 
 | _ #x s m i k H H' := 
   begin by_cases h: i ≤ x,
@@ -202,7 +307,7 @@ lemma subst_lift: ∀  {a}  (t : preterm L a) (s: term L) {m i k : ℕ} (H: i �
 | _ (func f)   _ _ _ _ _ _ := by refl
 | _ (fapp f t) _ _ _ _ _ _ := by simp* 
 
-lemma subst_subst: ∀ {a} (t : preterm L a) (s₁) {k₁}  (s₂) {k₂} (H : k₁ ≤ k₂), 
+lemma subst_subst: ∀ {a} (t : preterm 𝒮 a) (s₁) {k₁}  (s₂) {k₂} (H : k₁ ≤ k₂), 
     t[s₁ ⁄ k₁][s₂ ⁄ k₂] = t[s₂ ⁄ k₂ + 1][(s₁ [s₂ ⁄ k₂ - k₁]) ⁄ k₁] 
 | _ #x s₁ k₁ s₂ k₂ H := 
   begin apply decidable.lt_by_cases x k₁; intro h₁,
@@ -226,7 +331,7 @@ lemma subst_subst: ∀ {a} (t : preterm L a) (s₁) {k₁}  (s₂) {k₂} (H : k
 | _ (func f) _ _ _ _ _ := by refl
 | _ (fapp t s) _ _ _ _ _ := by simp*
 
-lemma subst_lift_by_lift : ∀{a} (t : preterm L a) (s : term L) (m i k : ℕ),
+lemma subst_lift_by_lift : ∀{a} (t : preterm 𝒮 a) (s : term 𝒮) (m i k : ℕ),
     (t ↑ m ＠ ( i + k + 1 ) ) [ (s ↑ m ＠ i) ⁄ k] = (t [ s ⁄ k ]) ↑ m ＠ (i+k)
 | _ #x s m i k :=
   begin by_cases h₁ : i + k + 1 ≤ x,
@@ -255,45 +360,45 @@ lemma subst_lift_by_lift : ∀{a} (t : preterm L a) (s : term L) (m i k : ℕ),
 | _ (func f)     _ _ _ _ := by refl
 | _ (fapp t₁ t₂) _ _ _ _ := by simp* 
 
-lemma subst_var0_lift : ∀{a} (t : preterm L a) (m i : ℕ), (t ↑ (m+1) ＠  (i+1) )[ #0 ⁄ i] = t ↑ m ＠ (i+1)
+lemma subst_var0_lift : ∀{a} (t : preterm 𝒮 a) (m i : ℕ), (t ↑ (m+1) ＠  (i+1) )[ #0 ⁄ i] = t ↑ m ＠ (i+1)
 | _ #x m i := begin apply decidable.lt_by_cases i x; intro h₀,
                 { have: i+1 ≤ x, by linarith,
-                have: ¬ (x + (m + 1) < i), by linarith, 
-                have: i < x + (m + 1), by linarith,
-                simp* , },
+                  have: ¬ (x + (m + 1) < i), by linarith, 
+                  have: i < x + (m + 1), by linarith,
+                  simp* , },
                 { subst h₀, simp , },
                 { have: ¬ (i + 1 ≤ x), by linarith, simp* , },
             end
 | _ (func f) _ _ := by refl
 | _ (fapp t s) _ _ := by simp* 
 
-
-@[simp, tls] lemma subst_var0_lift_by_1 {a} (t : preterm L a) (i : ℕ) : (t ↑ (1) ＠  (i+1) )[#0 ⁄ i] = t := 
+@[simp, tls] lemma subst_var0_lift_by_1 {a} (t : preterm 𝒮 a) (i : ℕ) : (t ↑ (1) ＠  (i+1) )[#0 ⁄ i] = t := 
 begin
     have h:= subst_var0_lift t 0 i,
     rw lift_by_0 at h,
     exact h,
 end
 
-@[simp, tls] lemma subst_for_0_lift_by_1: ∀ {a} (t : preterm L a) (s : term L) , (t ↑ 1 ＠ 0 )[s ⁄ 0] = t 
+@[simp, tls] lemma subst_for_0_lift_by_1: ∀ {a} (t : preterm 𝒮 a) (s : term 𝒮) , (t ↑ 1 ＠ 0 )[s ⁄ 0] = t 
 | _ #x _         := by refl
 | _ (func f) _   := by refl
 | _ (fapp t s) _ := by simp* 
 
 
 /--
-  Highest variable index occuring in a term (plus one).
+  Biggest (deepest) reference depth of variables occurring in a term (plus one).
 
   Examples:
   * `max_free_var #k = k+1` by definition.
   * `max_free_var t = 0` means no variables occur in `t`.
 -/
-def max_free_var: ∀ {a} (t : preterm L a), ℕ 
+def max_free_var: ∀ {a} (t : preterm 𝒮 a), ℕ 
 | _ #x := x+1
 | _ (func f)  := 0
 | _ (fapp t s) := max (max_free_var t) (max_free_var s)
 
-lemma trivial_lift_monotone {a} {t:preterm L a} {i j: ℕ} (h: i ≤ j) (H: t ↑ 1 ＠ i = t) : t ↑ 1 ＠ j = t :=
+/- If `t` is a fixpoint for lifting at `i`, then its a fixpoint for lifting at `j` for all `i≤j`  -/
+lemma trivial_lift_monotone {a} {t:preterm 𝒮 a} {i j: ℕ} (h: i ≤ j) (H: t ↑ 1 ＠ i = t) : t ↑ 1 ＠ j = t :=
 begin
   induction j with j,
   { rwa[le_zero_iff.mp h] at H,},
@@ -305,7 +410,7 @@ begin
   },
 end
 
-@[simp, tls] lemma lift_at_max_free_var {a} (t : preterm L a) : t ↑ 1 ＠ (max_free_var t) = t :=
+@[simp, tls] lemma lift_at_max_free_var {a} (t : preterm 𝒮 a) : t ↑ 1 ＠ (max_free_var t) = t :=
 begin
   induction t with T,
   { simp[max_free_var], },
@@ -319,69 +424,86 @@ begin
 end 
 
 end term
-variable (L)
+
+
+/-! ### formulas -/
+section formulas
+
+variable (𝒮)
 /--
-  `preformula L a` is a partially applied formula of first order predicate logic (with equality).
-  This definition includes symbols for falsum `⊥'`, equality `='`, implication `→'`, 
-  and `∧'`, or `∨'`, universal `∀'` and existential `∃'` quantifiers, a symbol `pred P`
-  for each predicate of the language `L` and `papp φ t` for applying a term `t`.
-  * For `a=0` this is a well-defined formula.
-  * For `a≠0` this is a partially applied predicate, requiring `a` more term applications to become
-    a well-formed formula.
+  `preformula 𝒮 a` is a partially applied formula of first-order logic over the signature `𝒮`. 
+  If applied to `a` terms it becomes a well-formed formula.
 -/
 inductive preformula : ℕ → Type u
 | bot                           : preformula 0
-| eq   ( t s : term L )         : preformula 0
+| eq   ( t s : term 𝒮 )         : preformula 0
 | imp  ( φ ψ : preformula 0 )   : preformula 0
 | and  ( φ ψ : preformula 0 )   : preformula 0
 | or   ( φ ψ : preformula 0 )   : preformula 0
 | all  ( φ : preformula 0 )     : preformula 0
 | ex   ( φ : preformula 0 )     : preformula 0 
-| pred { arity : ℕ } ( P : L.predicates arity )                  : preformula arity 
-| papp { arity : ℕ } ( φ : preformula (arity+1) ) ( t : term L ) : preformula arity
+| pred { arity : ℕ } ( P : 𝒮.pred_symb arity )                  : preformula arity 
+| papp { arity : ℕ } ( φ : preformula (arity+1) ) ( t : term 𝒮 ) : preformula arity
 
-@[reducible] def formula := preformula L 0
+@[reducible] def formula := preformula 𝒮 0
 
-variable {L}
+variable {𝒮}
 
-notation `⊥'` := preformula.bot 
+notation `⊥'`     := preformula.bot 
+infix ` =' `:100  := preformula.eq  
 
-infix ` =' `:100 := preformula.eq  
+infixr ` →' `:80  := preformula.imp
+infixr ` ∨' `:85  := preformula.or
+infixr ` ∧' `:90  := preformula.and 
 
-prefix `∀'`:110 := preformula.all
-prefix `∃'`:110 := preformula.ex 
+prefix `∀'`:110   := preformula.all
+prefix `∃'`:110   := preformula.ex 
 
-infixr ` →' `:80 := preformula.imp
-infixr ` ∨' `:85 := preformula.or
-infixr ` ∧' `:90 := preformula.and 
+@[simp] def preformula.iff (φ ψ : formula 𝒮) : formula 𝒮 := (φ →' ψ) ∧' (ψ  →' φ)
+infix ` ↔' `:70 := preformula.iff -- input \<=>
 
-@[simp] def iff (f₁ f₂ : formula L) : formula L := ( f₁ →' f₂ ) ∧'  ( f₂ →' f₁ )
-infix ` ↔' `:70 := iff -- input \<=>
+@[simp] def preformula.not (φ : formula 𝒮) : formula 𝒮 := (φ →' ⊥') 
+prefix `¬'`:115 := preformula.not
 
-@[simp] def not (f: formula L) : formula L := (f →' ⊥') 
-prefix `¬'`:115 := not
+def preformula.top : formula 𝒮  := ¬' ⊥'
+notation `⊤'` := preformula.top
 
-def top : formula L  := ¬' ⊥'
-notation `⊤'` := top
-
-#check ¬' (#0 =' #1)
 export preformula
 
-/- On De Bruijn indices:
-  
+/- 
+  ## Definition
+  The variables of a formula `φ` are by structural induction in the obvious way.
 
+  The variables at reference depth `k` or simply at `k` are defined 
+  by structural induction as follows:
+  - `⊥` and `pred P` have no variables at `k`
+  the variables at `k` of 
+  - `t=s`      are the variables at `k` of `t` and of `s`
+  - `φ □ ψ`    are the variables at `k` of `φ` and of `ψ` for `□ ∈ { → , ∧ , ∨ }`
+  - `papp φ t` are the variables at `k` of `φ` and of `t`
+  And most importantly 
+  - `□ φ`      are the variables at `k+1` of `φ` for `□ ∈ { ∀, ∃ }`
+
+  A variable of `φ` is called `k`-free if it is at a reference depth `≥k`.
+  
+  ## Remark
+  It follows that quantifiers act as another form of variable binders,
+  this time not just imagined. 
+  To define lifting (resp. substitution) of formulas we therefore need 
+  to increase the reference depth at which we lift (resp. substitute)
+  at whenever we cross a quantifier.
+
+  With this we can directly translate the lifting and substitution
+  lemmas of terms to formulas and their proofs will generally reduce to
+  the respective lemmas for terms (and some light arithmetic for crossing quantifiers).
 -/
+
+section lifts_and_substitutions
 
 namespace formula
 
-/--
-  `lift φ m i` increases the index of each _free_ variable greater or equal to `i` in `φ` by `m`.
-  Intuitively, this adds a batch of `m` new free variables
-  * Notation:  `φ ↑ m ＠ i`
-  * Note: We read this as "lift term `t` by `m` at `i`", which then informs the naming of later lemmas and our notation.
--/
-
-@[simp, reducible] def lift : ∀{a} , preformula L a → ℕ → ℕ → preformula L a 
+/-- `lift φ m i` increases the index of `i`-free variables in `φ` by `m`. -/
+@[simp, reducible] def lift : ∀{a} , preformula 𝒮 a → ℕ → ℕ → preformula 𝒮 a 
 | _ ⊥'  _ _         := ⊥'  
 | _ (t =' s) m i    := (term.lift t m i) =' (term.lift s m i)
 | _ ( φ →' ψ ) m i  := (lift φ m i) →' (lift ψ  m i)
@@ -391,77 +513,9 @@ namespace formula
 | _ ( ∃' φ ) m i    := ∃' (lift φ m (i+1))
 | _ (pred P) _ _    := pred P
 | _ (papp φ t) m i  := papp (lift φ m i) (term.lift t m i)
-end formula
 
-
-notation f ` ↑ `:90 m ` ＠ `:90 i :90 := formula.lift f m i
-notation f ` ↑₀ `:max n  := formula.lift f n 0
-
-#reduce #3 ↑ 3 ＠ 1
-#reduce (#3 =' #0) ↑ 3 ＠ 1
-
-namespace formula
-open preformula
-
-
-lemma all_lift {φ : formula L} {m i} : ∀'( φ ↑ m ＠ (i+1) ) = (∀' φ) ↑ m ＠ i := by refl
-
-
-@[simp, tls] lemma lift_by_0: ∀ {a} ( φ : preformula L a) {i}, φ ↑ 0 ＠ i = φ
-| _ ⊥' _            := by refl
-| _ (t =' s) _      := by simp
-| _ ( φ →' ψ ) _    := begin rw lift, congr; exact lift_by_0 _, end
-| _ ( φ ∧' ψ ) _    := begin rw lift, congr; exact lift_by_0 _, end
-| _ ( φ ∨' ψ ) _    := begin rw lift, congr; exact lift_by_0 _, end
-| _ ( ∀' φ ) _      := begin rw lift, congr, exact lift_by_0 φ, end
-| _ ( ∃' φ ) _      := begin rw lift, congr, exact lift_by_0 φ, end
-| _ ( pred P ) _    := by refl
-| _ ( papp φ t ) _  := begin rw lift, congr, exact lift_by_0 φ, exact term.lift_by_0 t, end
-
-
-lemma lift_lift: ∀{a} ( φ : preformula L a) (m) {i} (n) {j} ( H : j ≤ i ),
-    ( φ ↑ m ＠ i ) ↑ n ＠ j = ( φ ↑ n ＠ j) ↑ m ＠ (i+n)     -- lift(lift φ m i) n j = lift (lift φ  n j) m (i+n)
-| _ ⊥' _ _ _ _ _             := by refl
-| _ ( t =' s ) _ _ _ _ _     := by simp[*, term.lift_lift]
-| _ ( φ →' ψ ) _ _ _ _ _     := by simp[*]
-| _ ( φ ∧' ψ ) _ _ _ _ _     := by simp[*]
-| _ ( φ ∨' ψ ) _ _ _ _ _     := by simp[*]
-| _ ( ∀' φ ) _ _ _ _ _       := by simp[*, add_right_comm]
-| _ ( ∃' φ ) _ _ _ _ _       := by simp[*, add_right_comm]
-| _ ( pred P ) _ _ _ _ _     := by refl
-| _ ( papp φ t ) _ _ _ _ _   := by simp[*, term.lift_lift]
-
-lemma lift_lift_reverse {a} ( φ : preformula L a) {m i} (n) {j} (H : i + m ≤ j) :
-    ( φ ↑ m ＠ i ) ↑ n ＠ j = ( φ  ↑ n ＠  (j-m) ) ↑ m ＠ i := -- lift (lift f m i) n j = lift (lift f n (j-m)) m i
-begin
-    have h : i ≤ (j-m), from nat.le_sub_right_of_add_le H,
-    have h': m ≤ j, from (le_trans (m.le_add_left i) H),
-    rw [lift_lift φ n m h, nat.sub_add_cancel h'],
-end
-
-lemma lift_lift_merge: ∀ {a} ( φ : preformula L a ) {m i} (n) {j} (H : i ≤ j) (H' : j ≤ i + m),
-    ( φ ↑ m ＠ i ) ↑ n ＠ j = φ ↑ (m+n) ＠ i
-| _ ⊥' _ _ _ _ _ _           := by refl 
-| _ ( t =' s) _ _ _ _ _ _    := by simp[*, term.lift_lift_merge]
-| _ ( φ →' ψ ) _ _ _ _ _ _   := by simp[*]
-| _ ( φ ∧' ψ ) _ _ _ _ _ _   := by simp[*]
-| _ ( φ ∨' ψ ) _ _ _ _ _ _   := by simp[*]
-| _ ( ∀' φ ) _ _ _ _ _ _     := by simp[*, add_right_comm]
-| _ ( ∃' φ ) _ _ _ _ _ _     := by simp[*, add_right_comm]
-| _ ( pred P ) _ _ _ _ _ _   := by refl
-| _ ( papp φ t ) _ _ _ _ _ _ := by simp[*, term.lift_lift_merge]
-
-@[simp, tls] lemma lift_at_lift_merge {a} ( φ : preformula L a ) (m i n):
-    ( φ ↑ m ＠ i ) ↑ n ＠ i = φ ↑ (m+n) ＠ i := lift_lift_merge φ n (le_rfl) (i.le_add_right m)
-
-
-
-lemma lambda_lift_lift {a} (m) {i} (n) {j} (H : j≤i) : 
-    (λ ( φ :preformula L a),  ( φ ↑ m ＠ i ) ↑ n ＠ j ) = (λ φ, ( φ ↑ n ＠ j) ↑ m ＠ (i+n)) :=
-begin funext, apply lift_lift, exact H, end
-
-
-@[simp, tls] def subst :  ∀{a} , preformula L a → term L → ℕ → preformula L a
+/-- `subst t s k` substitutes `s ↑ k ＠ 0` for each variable at `k` in `t` -/
+@[simp, tls] def subst :  ∀{a} , preformula 𝒮 a → term 𝒮 → ℕ → preformula 𝒮 a
 | _ ⊥'  _ _         := ⊥'  
 | _ ( t₁ =' t₂) s k := (term.subst t₁ s k) =' (term.subst t₂ s k)
 | _ ( φ →' ψ ) s k  := (subst φ s k) →' (subst ψ  s k)
@@ -474,18 +528,71 @@ begin funext, apply lift_lift, exact H, end
 
 end formula
 
+
+notation f ` ↑ `:90 m ` ＠ `:90 i :90 := formula.lift f m i
 notation φ `[`:max t ` ⁄ `:95 n `]`:0 := formula.subst φ t n
 
-#reduce #5[#2 ⁄ 1]
-#reduce (#5 =' #4)[#0 ⁄ 5] 
- 
+-- #reduce #3 ↑ 3 ＠ 1
+-- #reduce (#3 =' #0) ↑ 3 ＠ 1
+-- #reduce #5[#2 ⁄ 1]
+-- #reduce (#5 =' #4)[#0 ⁄ 5] 
+
 namespace formula
 open preformula
 
--- lift and substitution lemmas for formulas; follow directly from the corresponding lemmas for terms
+-- lift and substitution lemmas for formulas
+@[simp, tls] lemma lift_by_0: ∀ {a} ( φ : preformula 𝒮 a) {i}, φ ↑ 0 ＠ i = φ
+| _ ⊥' _            := by refl
+| _ (t =' s) _      := by simp
+| _ ( φ →' ψ ) _    := begin rw lift, congr; exact lift_by_0 _, end
+| _ ( φ ∧' ψ ) _    := begin rw lift, congr; exact lift_by_0 _, end
+| _ ( φ ∨' ψ ) _    := begin rw lift, congr; exact lift_by_0 _, end
+| _ ( ∀' φ ) _      := begin rw lift, congr, exact lift_by_0 φ, end
+| _ ( ∃' φ ) _      := begin rw lift, congr, exact lift_by_0 φ, end
+| _ ( pred P ) _    := by refl
+| _ ( papp φ t ) _  := begin rw lift, congr, exact lift_by_0 φ, exact term.lift_by_0 t, end
 
-lemma lift_subst: ∀ {a}  ( φ : preformula L a) (s: term L) ( m i k : ℕ ) (h': i ≤ k),
-     φ[s ⁄ k]↑ m ＠ i = (φ ↑ m ＠  i)[s ⁄ (k+m)]  -- lift (subst f s k) m i = subst ( lift f m i) s (k+m)
+lemma lift_lift: ∀{a} ( φ : preformula 𝒮 a) (m) {i} (n) {j} ( H : j ≤ i ),
+    (φ ↑ m ＠ i) ↑ n ＠ j = (φ ↑ n ＠ j) ↑ m ＠ (i+n)   
+| _ ⊥' _ _ _ _ _             := by refl
+| _ ( t =' s ) _ _ _ _ _     := by simp[*, term.lift_lift]
+| _ ( φ →' ψ ) _ _ _ _ _     := by simp[*]
+| _ ( φ ∧' ψ ) _ _ _ _ _     := by simp[*]
+| _ ( φ ∨' ψ ) _ _ _ _ _     := by simp[*]
+| _ ( ∀' φ ) _ _ _ _ _       := by simp[*, add_right_comm]
+| _ ( ∃' φ ) _ _ _ _ _       := by simp[*, add_right_comm]
+| _ ( pred P ) _ _ _ _ _     := by refl
+| _ ( papp φ t ) _ _ _ _ _   := by simp[*, term.lift_lift]
+
+lemma lift_lift_reverse {a} ( φ : preformula 𝒮 a) {m i} (n) {j} (H : i + m ≤ j) :
+    (φ ↑ m ＠ i) ↑ n ＠ j = (φ  ↑ n ＠  (j-m)) ↑ m ＠ i := 
+begin
+    have h : i ≤ (j-m), from nat.le_sub_right_of_add_le H,
+    have h': m ≤ j, from (le_trans (m.le_add_left i) H),
+    rw [lift_lift φ n m h, nat.sub_add_cancel h'],
+end
+
+lemma lift_lift_merge: ∀ {a} ( φ : preformula 𝒮 a ) {m i} (n) {j} (H : i ≤ j) (H' : j ≤ i + m),
+    (φ ↑ m ＠ i) ↑ n ＠ j = φ ↑ (m+n) ＠ i
+| _ ⊥' _ _ _ _ _ _           := by refl 
+| _ ( t =' s) _ _ _ _ _ _    := by simp[*, term.lift_lift_merge]
+| _ ( φ →' ψ ) _ _ _ _ _ _   := by simp[*]
+| _ ( φ ∧' ψ ) _ _ _ _ _ _   := by simp[*]
+| _ ( φ ∨' ψ ) _ _ _ _ _ _   := by simp[*]
+| _ ( ∀' φ ) _ _ _ _ _ _     := by simp[*, add_right_comm]
+| _ ( ∃' φ ) _ _ _ _ _ _     := by simp[*, add_right_comm]
+| _ ( pred P ) _ _ _ _ _ _   := by refl
+| _ ( papp φ t ) _ _ _ _ _ _ := by simp[*, term.lift_lift_merge]
+
+@[simp, tls] lemma lift_at_lift_merge {a} ( φ : preformula 𝒮 a ) (m i n):
+    ( φ ↑ m ＠ i ) ↑ n ＠ i = φ ↑ (m+n) ＠ i := lift_lift_merge φ n (le_rfl) (i.le_add_right m)
+
+lemma lambda_lift_lift {a} (m) {i} (n) {j} (H : j≤i) : 
+    (λ ( φ :preformula 𝒮 a),  ( φ ↑ m ＠ i ) ↑ n ＠ j ) = (λ φ, ( φ ↑ n ＠ j) ↑ m ＠ (i+n)) :=
+begin funext, apply lift_lift, exact H, end
+
+lemma lift_subst: ∀ {a}  (φ : preformula 𝒮 a) (s: term 𝒮) ( m i k : ℕ ) (h': i ≤ k),
+     φ[s ⁄ k] ↑ m ＠ i = (φ ↑ m ＠  i)[s ⁄ (k+m)]  
 | _ ⊥' _ _ _ _ _            := by refl
 | _ (t₁ =' t₂) _ _ _ _ _    := by simp[*, term.lift_subst]
 | _ ( φ →' ψ ) _ _ _ _ _    := by simp[*]
@@ -496,8 +603,8 @@ lemma lift_subst: ∀ {a}  ( φ : preformula L a) (s: term L) ( m i k : ℕ ) (h
 | _ ( pred P ) _ _ _ _ _    := by refl
 | _ ( papp φ t ) _ _ _ _ _  := by simp[*, term.lift_subst]
 
-lemma subst_lift : ∀ {a}  ( φ : preformula L a) (s: term L) {m i k : ℕ } (H: i ≤ k) (H' : k ≤ i + m),
-    ( φ ↑ (m+1) ＠ i )[ s ⁄ k ] = φ ↑ m ＠ i -- subst ( lift f (m+1) i) s k = lift f m i
+lemma subst_lift : ∀ {a}  ( φ : preformula 𝒮 a) (s: term 𝒮) {m i k : ℕ } (H: i ≤ k) (H' : k ≤ i + m),
+    (φ ↑ (m+1) ＠ i)[s ⁄ k] = φ ↑ m ＠ i 
 | _ ⊥' _ _ _ _ _ _          := by refl
 | _ (t₁ =' t₂) _ _ _ _ _ _  := by simp[*, term.subst_lift]
 | _ ( φ →' ψ ) _ _ _ _ _ _  := by simp[*]
@@ -508,9 +615,8 @@ lemma subst_lift : ∀ {a}  ( φ : preformula L a) (s: term L) {m i k : ℕ } (H
 | _ (pred P) _ _ _ _ _ _    := by refl
 | _ ( papp φ t) _ _ _ _ _ _ := by simp[*, term.subst_lift]
 
-lemma subst_subst : ∀ {a} ( φ : preformula L a) (s₁) {k₁} (s₂) {k₂} ( H : k₁ ≤ k₂ ), 
+lemma subst_subst : ∀ {a} ( φ : preformula 𝒮 a) (s₁) {k₁} (s₂) {k₂} ( H : k₁ ≤ k₂ ), 
     φ [ s₁ ⁄ k₁] [ s₂ ⁄ k₂] = φ [ s₂ ⁄ k₂ + 1] [ (s₁ [s₂ ⁄ k₂ - k₁] ) ⁄ k₁ ] 
-    -- subst ( subst f s₁ i) s₂ j = subst (subst f s₂ (j+1)) (subst s₁ s₂ (j-i) ) i
 | _ ⊥' _ _ _ _ _            := by refl
 | _ (t₁ =' t₂) _ _ _ _ _    := by simp[*, term.subst_subst]
 | _ ( φ →' ψ ) _ _ _ _ _    := by simp[*]
@@ -521,9 +627,8 @@ lemma subst_subst : ∀ {a} ( φ : preformula L a) (s₁) {k₁} (s₂) {k₂} (
 | _ (pred P) _ _ _ _ _      := by refl
 | _ (papp φ t) _ _ _ _ _    := by simp[*, term.subst_subst]
 
-
-lemma subst_lift_in_lift : ∀{a} ( φ : preformula L a) (s : term L) (m i k),
-    (φ ↑ m ＠ (i + k + 1)) [ (s ↑ m ＠ i) ⁄ k] = φ[s ⁄ k] ↑ m ＠ (i+k) --subst (lift f m (i + k + 1)) (lift s m i) k = lift (subst f s k) m (i + k)
+lemma subst_lift_in_lift : ∀{a} ( φ : preformula 𝒮 a) (s : term 𝒮) (m i k),
+    (φ ↑ m ＠ (i + k + 1)) [ (s ↑ m ＠ i) ⁄ k] = φ[s ⁄ k] ↑ m ＠ (i+k) 
 | _ ⊥' _ _ _ _          := by refl
 | _ (t₁ =' t₂) _ _ _ _  := by simp[*, term.subst_lift_by_lift]
 | _ ( φ →' ψ ) _ _ _ _  := by simp[*]
@@ -534,17 +639,15 @@ lemma subst_lift_in_lift : ∀{a} ( φ : preformula L a) (s : term L) (m i k),
 | _ (pred P) _ _ _ _    := by refl
 | _ (papp φ t) _ _ _ _  := by simp[*, term.subst_lift_by_lift]
 
--- lemma subst0_subst_formula {a} (φ : preformula L a) (s₁ s₂ : term L) (k₂):
---     φ [ s₁ ⁄ 0] [ s₂ ⁄ k₂] = φ [ s₂ ⁄ k₂ + 1] [ (s₁ [s₂ ⁄ k₂ ] ) ⁄ 0 ] := subst_subst φ s₁ s₂ (k₂.zero_le)
 
-@[tls] lemma subst0_lift_by_lift {a}  (φ : preformula L a) {s : term L} {m i:ℕ } :
-    (φ ↑ m ＠ (i + 1) ) [ (s ↑ m ＠ i) ⁄ 0] = φ[s ⁄ 0] ↑ m ＠ i := subst_lift_in_lift φ s m i 0
+@[tls] lemma subst0_lift_by_lift {a}  (φ : preformula 𝒮 a) {s : term 𝒮} {m i:ℕ } :
+    (φ ↑ m ＠ (i + 1)) [(s ↑ m ＠ i) ⁄ 0] = φ[s ⁄ 0] ↑ m ＠ i := subst_lift_in_lift φ s m i 0
 
+@[tls] lemma subst_at_lift {a} (φ : preformula 𝒮 a) (m) (s : term 𝒮) (k) : 
+  (φ ↑ (m+1) ＠ k)[s ⁄ k] =  φ ↑ m ＠ k := subst_lift φ s (le_refl k) (le.intro rfl)
 
-@[tls] lemma subst_at_lift {a} (φ  : preformula L a) (m) (s : term L) (k)  : ( φ ↑ (m+1) ＠  k)[s ⁄ k] =  φ ↑ m ＠ k
-    := subst_lift φ s (le_refl k) (le.intro rfl)
-
-@[tls] lemma subst_var0_lift : ∀{a} (φ : preformula L a) (m i : ℕ), (φ ↑ (m+1) ＠  (i+1) )[ #0 ⁄ i] = φ ↑ m ＠ (i+1)
+@[tls] lemma subst_var0_lift : ∀{a} (φ : preformula 𝒮 a) (m i : ℕ), 
+  (φ ↑ (m+1) ＠ (i+1))[#0 ⁄ i] = φ ↑ m ＠ (i+1)
 | _ ⊥'  _ _         := by refl 
 | _ ( t₁ =' t₂) m i := by simp[term.subst_var0_lift]
 | _ ( φ →' ψ ) m i  := by simp*
@@ -555,17 +658,18 @@ lemma subst_lift_in_lift : ∀{a} ( φ : preformula L a) (s : term L) (m i k),
 | _ (pred P) _ _    := by refl
 | _ (papp φ t) m i  := by simp[*, term.subst_var0_lift]
 
-@[tls] lemma subst_var0_lift_by_1 {a}  (φ : preformula L a)  (i : ℕ) : (φ ↑ 1 ＠  (i+1) )[#0 ⁄ i] = φ := 
+@[tls] lemma subst_var0_lift_by_1 {a}  (φ : preformula 𝒮 a)  (i : ℕ) : 
+  (φ ↑ 1 ＠ (i+1))[#0 ⁄ i] = φ := 
 begin
   have h:= subst_var0_lift φ 0 i,
   rwa lift_by_0 at h,
 end
 
-lemma subst_var0_for_0_lift_by_1{a}  (φ : preformula L a) : (φ ↑ 1 ＠ 1 )[#0 ⁄ 0] = φ := subst_var0_lift_by_1 φ 0
+@[tls] lemma subst_var0_for_0_lift_by_1 {a} (φ : preformula 𝒮 a) : 
+  (φ ↑ 1 ＠ 1)[#0 ⁄ 0] = φ := subst_var0_lift_by_1 φ 0
 
-
-
-@[simp, tls] lemma subst_for_0_lift_by_1: ∀ {a} ( φ : preformula L a) (s : term L), (φ ↑ 1 ＠ 0 )[s ⁄ 0] = φ 
+@[simp, tls] lemma subst_for_0_lift_by_1: ∀ {a} ( φ : preformula 𝒮 a) (s : term 𝒮), 
+  (φ ↑ 1 ＠ 0 )[s ⁄ 0] = φ 
 | _ ⊥' _          := by refl
 | _ (t₁ =' t₂) _  := by simp[*, term.subst_for_0_lift_by_1]
 | _ ( φ →' ψ ) _  := by simp[*]
@@ -576,8 +680,8 @@ lemma subst_var0_for_0_lift_by_1{a}  (φ : preformula L a) : (φ ↑ 1 ＠ 1 )[#
 | _ (pred P) _    := by refl
 | _ (papp φ t) _  := by simp[*, term.subst_lift_by_lift]
 
--- a  i-closed formula is j-closed for j≥i
-lemma trivial_lift_monotone {a} {φ : preformula L a} {i j} 
+/- If `φ` is a fixpoint for lifting at `i`, then its a fixpoint for lifting at `j` for all `i≤j`  -/
+lemma trivial_lift_monotone {a} {φ : preformula 𝒮 a} {i j} 
   (H : φ ↑ 1 ＠ i = φ) (h : i ≤ j) : φ ↑ 1 ＠ j = φ :=
 begin
   induction j with j,
@@ -589,29 +693,34 @@ begin
       rw [←H, ←lift_lift φ 1 1 h₁, h₂], }, },
 end 
 
+
+
 /--
-  `alls k φ` is the formula obtained by binding the the first `k` free variables in `φ` with universal quantifiers.
+  `alls k φ` is the formula obtained by binding the the first `k` free variables in `φ` 
+  with universal quantifiers. 
+  
+  In other words, we add `k` universal quantifier in from of `φ`
 -/
-def alls : ∀ (k:ℕ) (φ: formula L) , formula L
+def alls : ∀ (k:ℕ) (φ: formula 𝒮) , formula 𝒮
 | 0     φ   := φ 
 | (k+1) φ   := ∀' (alls k φ )
 
-lemma all_alls: ∀ (φ: formula L) (k:ℕ) , ∀' (alls k φ) = alls k (∀'φ) 
+-- lemmas about alls
+lemma all_alls: ∀ (φ: formula 𝒮) (k:ℕ) , ∀' (alls k φ) = alls k (∀'φ) 
 | φ 0 := by refl
 | φ (k+1) := begin unfold alls, congr' 1, apply all_alls, end
 
-lemma alls_succ (k) (φ : formula L) : alls (k+1) φ = alls k (∀' φ) := begin rw [alls, all_alls], end
+lemma alls_succ (k) (φ : formula 𝒮) : alls (k+1) φ = alls k (∀' φ) := begin rw [alls, all_alls], end
 
-
-lemma alls_alls: ∀ (φ: formula L) (m n:ℕ) , alls n (alls m φ) = alls m (alls n φ)
+lemma alls_alls: ∀ (φ: formula 𝒮) (m n:ℕ) , alls n (alls m φ) = alls m (alls n φ)
 | φ 0 n := by refl
 | φ (m+1) n := begin rw alls, rw ←all_alls _ _, rw alls_alls _ m n, refl, end
 
-lemma alls_lift : ∀  (φ: formula L) (m i n:ℕ), alls n (φ ↑ m ＠ (i+n)) = (alls n φ) ↑ m ＠ i
+lemma alls_lift : ∀  (φ: formula 𝒮) (m i n:ℕ), alls n (φ ↑ m ＠ (i+n)) = (alls n φ) ↑ m ＠ i
 | φ m i 0 := by refl
 | φ m i (n+1) := begin dsimp[alls], congr, rw ←succ_add_eq_succ_add i n, apply alls_lift,end
 
-lemma alls_at_lift  (φ: formula L) (m n:ℕ) : alls n (φ ↑ m ＠ n) = (alls n φ) ↑ m ＠ 0 :=
+lemma alls_at_lift  (φ: formula 𝒮) (m n:ℕ) : alls n (φ ↑ m ＠ n) = (alls n φ) ↑ m ＠ 0 :=
 begin 
   let h := alls_lift φ m 0 n, 
   rwa zero_add at h, 
@@ -620,75 +729,87 @@ end
 /--
   `substs k i j φ` is the formula `φ[#(k+i) ⁄ k+j]...[#(1+i) ⁄ 1+j][#i ⁄ j]`.
 -/
-def substs : ∀(k i j: ℕ ) ( φ: formula L), formula L
+def substs : ∀(k i j: ℕ ) ( φ: formula 𝒮), formula 𝒮
 | 0 i j φ  := φ 
 | (k+1) i j φ := substs k i j (φ [#(k+i) ⁄ (k+j)])
 
-lemma substs_succ (k i j: ℕ ) (φ : formula L): substs (k+1) i j φ = (substs k (i+1) (j+1) φ) [ #i ⁄ j] :=
+-- lemmas about substs
+lemma substs_succ (k i j: ℕ ) (φ : formula 𝒮): substs (k+1) i j φ = (substs k (i+1) (j+1) φ) [ #i ⁄ j] :=
 begin
   induction k generalizing φ,
   { simp[substs] },
   { simp[*,substs, succ_add_eq_succ_add] }
 end 
 
-lemma all_substs {k i j}{φ : formula L} : ∀'(substs k i (j+1) φ) = substs k i j ∀'φ :=
+lemma all_substs {k i j}{φ : formula 𝒮} : 
+  ∀'(substs k i (j+1) φ) = substs k i j ∀'φ :=
 begin
-    induction k generalizing φ,
-    { dsimp[substs], refl },
-    { simp[*,substs, succ_add_eq_succ_add, add_assoc] }
+  induction k generalizing φ,
+  { dsimp[substs], refl },
+  { simp[*,substs, succ_add_eq_succ_add, add_assoc] }
 end
 
+/-
+  ## Remark
+  In the future we need to be able define 
+    
+    "a formula `φ` with free variables among x₀,...,xₖ"
 
--- we need to be able to talk about formulas φ( x_1 , ... , x_n) with free variables among x_1, ... , x_n
--- wlog #n is the "outermost" (i.e. the highest) free variable in our De Bruijn representation of φ
--- then lifting φ at n+1 does not change the formula
--- thus we obtain the following definition
-/--
-  A formula `φ` is `k`-closed if lifting `φ ↑ 1 ＠ k` is the identity. 
+  in our de Bruijn representation of variables.
+  One possible solution is to say that `φ` has no 
+  `k+1`-free variables by traversing inductive definition,
+  to check if each variable is of not `k+1`-free.
 
-  Intuitively this means that `φ` has free variables among `x₁ ... xₖ`.
+  However, we have already developed a more convenient tool
+  in form of lifting. 
+  If `φ` has no `k+1`-free variables then lifting at `k+1` 
+  does not change the formula.
+  We will see that this serves as an adequate definition
+  for our purposes.
 -/
-@[simp, reducible] def closed {a} (k : ℕ) ( φ : preformula L a) := φ ↑ 1 ＠ k = φ 
 
 /--
-  A sentence is a `0`-closed formula, i.e. a formula without free variables.
+  A formula `φ` is `k`-closed if it has no `k`-free variables,
+  i.e. if lifting at `k` does not change the formula.
 -/
-@[simp, reducible] def sentence (φ  : formula L) := closed 0 φ 
+@[simp, reducible] def closed {a} (k : ℕ) ( φ : preformula 𝒮 a) := φ ↑ 1 ＠ k = φ 
+
+/-- A sentence is a `0`-closed formula, i.e. a formula without free variables. -/
+@[simp, reducible] def sentence (φ : formula 𝒮) := closed 0 φ 
 postfix ` is_sentence'`:max := sentence
 
--- quantification of closed formulas
-lemma closed_all {φ : formula L} {k} (H : closed (k+1) φ) : closed k (∀' φ) :=
-begin
-  dsimp, congr, exact H,
-end
+-- various lemmas involving lifts and substitutions of closed formulas
 
-lemma closed_ex  {φ : formula L} {k} (H : closed (k+1) φ) : closed k (∃' φ) :=
-begin
-  dsimp, congr, exact H,
-end
+lemma closed_all {φ : formula 𝒮} {k} (H : closed (k+1) φ) : closed k (∀' φ) :=
+begin dsimp, congr, exact H, end
 
--- lifting a k-closed formula at l ≥ k is trivial
-lemma lift_closed_id_h { φ : formula L} {k} (H : closed k φ) (m i) : φ ↑ m ＠ (k+i) = φ :=
+lemma closed_ex  {φ : formula 𝒮} {k} (H : closed (k+1) φ) : closed k (∃' φ) :=
+begin dsimp, congr, exact H end
+
+lemma lift_closed_id_h { φ : formula 𝒮} {k} (H : closed k φ) (m i) : 
+  φ ↑ m ＠ (k+i) = φ :=
 begin
   induction m generalizing φ,
   { apply lift_by_0, },
   { rw [succ_eq_add_one, ←lift_lift_merge φ 1 (le_refl _ ) (le.intro rfl), m_ih H],
-    apply trivial_lift_monotone H (le.intro rfl) ,
-  },
+    apply trivial_lift_monotone H (le.intro rfl) },
 end
 
-lemma lift_closed_id { φ : formula L} {k} (H : closed k φ) (m) {l} (h : k ≤ l): (φ ↑ m ＠ l) = φ :=
+-- `k`-closed formulas are fixpoints for lifts at reference depth `≥k`
+lemma lift_closed_id { φ : formula 𝒮} {k} (H : closed k φ) (m) {l} (h : k ≤ l): 
+  (φ ↑ m ＠ l) = φ :=
 begin
-    cases le_iff_exists_add.mp h with i h_i,
-    subst h_i, exact lift_closed_id_h H m i,
+  cases le_iff_exists_add.mp h with i h_i,
+  subst h_i, 
+  exact lift_closed_id_h H m i,
 end
 
--- lifting (a set of) sentences is always trivial
-lemma lift_sentence_id {x: formula L} (H: sentence x) { m i } :  (x ↑ m ＠ i) = x 
-  := lift_closed_id H m (i.zero_le)
+-- sentences are fixpoints of all lifts 
+lemma lift_sentence_id {φ : formula 𝒮} (H: sentence φ) { m i } : 
+  (φ ↑ m ＠ i) = φ := lift_closed_id H m (i.zero_le)
 
-lemma lift_set_of_sentences_id {Γ : set $ formula L} (H : ∀ ϕ ∈ Γ, sentence ϕ) {m i} 
-  : (λ ϕ: formula L, ϕ ↑ m ＠ i) '' Γ = Γ :=
+lemma lift_set_of_sentences_id {Γ : set $ formula 𝒮} (H : ∀ ϕ ∈ Γ, sentence ϕ) {m i} 
+  : (λ ϕ: formula 𝒮, ϕ ↑ m ＠ i) '' Γ = Γ :=
 begin
   apply ext, intro x,
   apply iff.intro,
@@ -700,25 +821,26 @@ begin
   { intro h, rw mem_image_eq, use x, exact ⟨h, lift_sentence_id (H x h)⟩, },
 end
 
--- substituting in a k-closed formula the l-th free variable with l ≥ k is trivial
-lemma subst_closed_id_h { φ : formula L} (t:term L)  {k} (i) ( H : closed k φ) : (φ [t ⁄ k+i]) = φ :=
+
+lemma subst_closed_id_h { φ : formula 𝒮} (t:term 𝒮) {k} (i) ( H : closed k φ) : 
+  (φ [t ⁄ k+i]) = φ :=
 begin
   have h := subst_at_lift φ 0 t (k+i),
   repeat {rwa lift_closed_id_h H _ _ at h,},
 end
 
-lemma subst_closed_id {φ : formula L}{i}  (H : closed i φ)  (t:term L) {k} (h : i≤k) : (φ [t ⁄ k]) = φ :=
+-- `k`-closed formulas are fixpoints for substitutions at reference depth `≥k`
+lemma subst_closed_id {φ : formula 𝒮}{i}  (H : closed i φ)  (t:term 𝒮) {k} (h : i≤k) : (φ [t ⁄ k]) = φ :=
 begin
   cases le_iff_exists_add.mp h with j h_j,
   subst h_j, exact subst_closed_id_h t j H,
 end
 
--- substituting in (a set of) sentences is always trivial
-lemma subst_sentence_id { φ : formula L} ( H : sentence φ )  {t: term L} {k:ℕ} :  (φ [t ⁄ k]) = φ 
+lemma subst_sentence_id { φ : formula 𝒮} ( H : sentence φ )  {t: term 𝒮} {k:ℕ} :  (φ [t ⁄ k]) = φ 
   := subst_closed_id H t (k.zero_le)
 
-lemma subst_set_of_sentences_id {Γ : set $ formula L} {t k} (H : ∀f ∈ Γ, sentence f)
-  : (λ (ϕ: formula L), ϕ[t ⁄ k]) '' Γ = Γ :=
+lemma subst_set_of_sentences_id {Γ : set $ formula 𝒮} {t k} (H : ∀f ∈ Γ, sentence f)
+  : (λ (ϕ: formula 𝒮), ϕ[t ⁄ k]) '' Γ = Γ :=
 begin
   apply ext, intro x,
   apply iff.intro,
@@ -731,10 +853,11 @@ begin
 end
 
 /--
-  Intuitively, `max_free_var φ = 0` means that `φ` has no free variables,
-  while  `max_free_var φ = k+1` means that `xₖ` is a free variable of `φ`.
+  Biggest (deepest) reference depth of variables occurring in a formula (plus one).
+
+  If equal to `0` the formula has no free variables.
 -/
-def max_free_var :  ∀ {a} (φ: preformula L a), ℕ 
+def max_free_var :  ∀ {a} (φ: preformula 𝒮 a), ℕ 
 | _ ⊥'           := 0
 | _ (t₁ =' t₂)   := max (term.max_free_var t₁) ( term.max_free_var t₂)
 | _ ( ∀'φ )      := (max_free_var φ) - 1
@@ -745,8 +868,8 @@ def max_free_var :  ∀ {a} (φ: preformula L a), ℕ
 | _ (pred P)     := 0
 | _ (papp φ t)   := max (max_free_var φ) ( term.max_free_var t )
 
--- The above intuition tells us that every formula should be closed at its maximal free variable 
-lemma closed_max_free_var {a} (φ : preformula L a) : closed (max_free_var φ) φ :=
+/- This lemma shows that our definition of closed is exactly what our intuition tells us. -/
+lemma closed_max_free_var {a} (φ : preformula 𝒮 a) : closed (max_free_var φ) φ :=
 begin
   unfold closed,
   induction φ,
@@ -774,13 +897,11 @@ begin
 end 
 
 /--
-  The (universal) closure of a `k`-closed formula.
-  Intuitively, given a formula `φ` with free variables among `x₁ ... xₖ` 
-  the closure is `∀xₖ ... ∀x₁ φ`. 
+  The (universal) closure of a `k`-closed formula, binding its free variables.
 -/
-@[reducible] def closure (φ: formula L) {k} (H: closed k φ) := alls k φ
+@[reducible] def closure (φ: formula 𝒮) {k} (H: closed k φ) := alls k φ
 
-lemma closure_is_sentence  { φ : formula L} {k} (H : closed k φ) : (closure φ H) is_sentence' :=
+lemma closure_is_sentence  { φ : formula 𝒮} {k} (H : closed k φ) : (closure φ H) is_sentence' :=
 begin
   induction k generalizing φ,
   { exact H, },
@@ -789,21 +910,37 @@ begin
     exact k_ih (closed_all H), },
 end
 
-lemma lambda_lift_subst_formula {a} {s: term L} { m i k : ℕ } (h': i ≤ k) 
-  : (λ (ϕ: preformula L a), lift (subst ϕ s k) m i) = (λ ϕ, subst ( lift ϕ m i) s (k+m)) :=
+lemma lambda_lift_subst_formula {a} {s: term 𝒮} { m i k : ℕ } (h': i ≤ k) 
+  : (λ (ϕ: preformula 𝒮 a), lift (subst ϕ s k) m i) = (λ ϕ, subst ( lift ϕ m i) s (k+m)) :=
 begin funext, apply lift_subst, assumption, end
 
+-- /-- Lift operation on sets of formulas. -/
+-- @[simp] def lift_set (Γ : set $ formula 𝒮) (m i) : set $ formula 𝒮 := ((λ (ϕ : formula 𝒮), ϕ ↑ m ＠ i) '' Γ)
+-- /-- Substitution operation on sets of formulas. -/
+-- @[simp] def subst_set  (Γ : set $ formula 𝒮) (s k) : set $ formula 𝒮 := ((λ (ϕ : formula 𝒮), ϕ [s ⁄ k]) '' Γ)
+
 end formula
+
+end lifts_and_substitutions
+
+end formulas
+
 export formula
+
+/-!### Proof terms of natural deduction -/
+section proof_terms
 
 local notation φ :: Γ := insert φ Γ 
 
 /--
-  An implementation of a Natural Deduction proof system for intuitionistic first-order predicate logic
-  with equality.
+  An intuitionistic natural deduction proof calculus 
+  for first order predicate logic with rules for equality 
+
+  Fresh variables for universal quantifier introduction and existential quantifier elimination
+  are introduced by lifting. 
 -/
 
-inductive proof : (set $ formula L) → formula L → Type u
+inductive proof : (set $ formula 𝒮) → formula 𝒮 → Type u
 | hypI {Γ} {φ} (h : φ ∈ Γ) : proof Γ φ 
 | botE {Γ} {φ} (H : proof Γ  ⊥' ) : proof Γ φ
 -- implication
@@ -817,76 +954,146 @@ inductive proof : (set $ formula L) → formula L → Type u
 -- disjunction
 | orI₁ {Γ} {φ ψ} (H : proof Γ φ) : proof Γ (φ ∨' ψ)
 | orI₂ {Γ} {φ ψ} (H : proof Γ ψ) : proof Γ (φ ∨' ψ)
-| orE  {Γ}  (φ ψ) {χ} (H  : proof Γ (φ ∨' ψ)) 
-                      (H₁ : proof (φ::Γ) χ) 
-                      (H₂ : proof (ψ::Γ) χ) : proof Γ χ
--- quanitfication
-| allI  {Γ} {φ} (H : proof ( (λ (ϕ:formula L) , ϕ ↑₀ 1) '' Γ ) φ) : proof Γ (∀'φ)
+| orE  {Γ}  (φ ψ) {χ} (H  : proof Γ (φ ∨' ψ))  
+                      (H₁ : proof (φ :: Γ) χ) 
+                      (H₂ : proof (ψ :: Γ) χ) : proof Γ χ
+-- quantification
+| allI  {Γ} {φ} (H : proof ((λ ϕ, ϕ ↑ 1 ＠ 0) '' Γ) φ) : proof Γ (∀'φ)
 | allE  {Γ} (φ) {t} (H : proof Γ (∀'φ)) : proof Γ (φ [t ⁄ 0])
 | exI   {Γ φ} (t) (H : proof Γ (φ[t ⁄ 0])) : proof Γ  (∃'φ)
 | exE   {Γ ψ} (φ) (H₁ : proof Γ (∃'φ) ) 
-                  (H₂ : proof ( φ :: ((λ (ϕ: formula L) , ϕ ↑₀ 1) '' Γ) ) (ψ ↑₀ 1)) : proof Γ ψ
+  (H₂ : proof  (φ :: (λ ϕ, ϕ ↑ 1 ＠ 0) '' Γ) (ψ ↑ 1 ＠ 0)) : proof Γ ψ
 -- equality
 | eqI {Γ} (t) : proof Γ (t =' t)
 | eqE {Γ} {s t φ } (H₁ : proof Γ (s =' t)) (H₂ : proof Γ (φ[s ⁄ 0])) : proof Γ (φ [t ⁄ 0])
 infix ` ⊢ `:55 := proof 
 
+/-
+  The deduction rules for quantifiers deserve some explanation.
+ 
+   Γ ⊢ φ[x₀/x] 
+  -------------∀x_I
+    Γ ⊢ ∀x φ 
+
+  with x₀ a variable fresh for Γ.
+
+  Often the context is kept implicit in which case the rule stated as
+
+  ----------- 
+  | x₀      |
+  |   ...   |
+  | φ[x₀/x] |
+  ----------- ∀x_I    x₀ does not occur outside the indicated box
+    Γ ⊢ ∀x φ 
+  
+  In our de Bruijn representation we can introduce a fresh variable  at `0` 
+  by lifting both Γ and ∀φ by `1`. The lower proof term then reads
+
+    `Γ ↑ 1 ＠ 0  ⊢ (∀φ) ↑  1 ＠  0`
+
+  and by definition  
+
+    `(∀φ) ↑  1 ＠  0  = ∀(φ ↑ 1 ＠ 1)`.
+
+  This allows us to apply the above deduction rule for our fresh variable `#0` results in
+
+    `Γ ↑ 1 ＠ 0  ⊢ (φ ↑  1 ＠ 1) [#0 ⁄ 0] `.
+
+  By `subst_var0_for_0_lift_by_1` this simplifies to
+    
+    `Γ ↑ 1 ＠ 0  ⊢ φ`
+
+  and we arrive at our universal introduction.
+
+  Similarly, existential elimination is defined as   
+
+    Γ ⊢ ∃x φ   φ[x₀/x] :: Γ ⊢ ψ      
+    ---------------------------- ∃x_E  
+              Γ ⊢ ψ
+
+  with x₀ a variable fresh for φ, ψ and Γ,
+  or with context kept implicit
+
+            --------------
+            | x₀ φ[x₀/x] |
+            |    ...     |
+    ∃x φ    |     ψ      |      
+    ---------------------- ∃x_E   x₀ does not occur outside the indicated box.
+             ψ
+
+  This time we introduce a fresh variable by lifting `Γ`, `ψ` and `∃φ`. 
+  Again, by definition 
+  
+    `(∃φ) ↑ 1 ＠  0  = ∃(φ ↑  1 ＠ 1)` 
+
+  and to apply the above described deduction rule we need a proof term of the form
+
+   ` (φ ↑  1 ＠ 1) [#0 ⁄ 0] :: (Γ ↑ 1 ＠ 0) ⊢ (ψ ↑ 1 ＠ 0)`
+
+  which by `subst_var0_for_0_lift_by_1`, simplifies to 
+
+    ` φ :: (Γ ↑ 1 ＠ 0) ⊢ (ψ ↑ 1 ＠ 0)`.
+    
+  But this is how we defined existential elimination.
+-/
+
 /-- 
   `provable Γ φ` says that there exists a proof of `φ` under the hypotheses in `Γ`,
   i.e. it is a fancy way to say that the type `Γ ⊢ φ` is non-empty. 
 -/
-def provable (φ : formula L) (Γ)  : Prop := nonempty (Γ ⊢ φ)
+def provable (φ : formula 𝒮) (Γ)  : Prop := nonempty (Γ ⊢ φ)
 infix ` is_provable_within `:100 := provable
 
 /--
   The law of excluded middle for when we want to argue in classical logic.
 -/
-def lem : set $ formula L := { (φ ∨' ¬'φ) |  (φ: formula L) (h: φ is_sentence') } -- do we need the extra condition?
+def lem : set $ formula 𝒮 := { (φ ∨' ¬'φ) |  (φ: formula 𝒮) (h: φ is_sentence') } -- do we need the extra condition?
+
 namespace proof
 /--
   Rule for weakening the context of a proof by allowing more premises.
 -/
-def weak {Δ φ}  (Γ: set $ formula L ) ( H : Γ ⊢ φ ) (h: Γ ⊆ Δ): (Δ ⊢ φ) :=
+def weak {Δ φ}  (Γ: set $ formula 𝒮 ) ( H : Γ ⊢ φ ) (h: Γ ⊆ Δ): (Δ ⊢ φ) :=
 begin
-    induction H generalizing Δ,
-    { apply hypI (h H_h) },
-    { apply botE, apply H_ih, assumption },
+  induction H generalizing Δ,
+  { apply hypI (h H_h) },
+  { apply botE, apply H_ih, assumption },
 
-    { apply impI, apply H_ih, apply insert_subset_insert, assumption },
-    { apply impE, apply H_ih_H₁, assumption, 
-      apply H_ih_H₂, assumption },
+  { apply impI, apply H_ih, apply insert_subset_insert, assumption },
+  { apply impE, apply H_ih_H₁, assumption, 
+    apply H_ih_H₂, assumption },
 
-    { apply andI,  apply H_ih_H₁, exact h, 
-      apply H_ih_H₂, exact h},
-    { apply andE₁, apply H_ih, exact h },
-    { apply andE₂, apply H_ih, exact h },
+  { apply andI,  apply H_ih_H₁, exact h, 
+    apply H_ih_H₂, exact h},
+  { apply andE₁, apply H_ih, exact h },
+  { apply andE₂, apply H_ih, exact h },
 
-    { apply orI₁, apply H_ih, exact h, },
-    { apply orI₂, apply H_ih, exact h, },
-    { apply orE,  apply H_ih_H, exact h, 
-      apply H_ih_H₁, apply insert_subset_insert, exact h, 
-      apply H_ih_H₂, apply insert_subset_insert, exact h},
+  { apply orI₁, apply H_ih, exact h, },
+  { apply orI₂, apply H_ih, exact h, },
+  { apply orE,  apply H_ih_H, exact h, 
+    apply H_ih_H₁, apply insert_subset_insert, exact h, 
+    apply H_ih_H₂, apply insert_subset_insert, exact h},
 
-    { apply allI, apply H_ih, exact image_subset _ h,},
-    { apply allE, apply H_ih, exact h},
+  { apply allI, apply H_ih, exact image_subset _ h,},
+  { apply allE, apply H_ih, exact h},
 
-    { apply exI, apply H_ih, exact h},
-    { apply exE, apply H_ih_H₁, exact h, 
-      apply H_ih_H₂, apply insert_subset_insert, exact image_subset _ h,},
+  { apply exI, apply H_ih, exact h},
+  { apply exE, apply H_ih_H₁, exact h, 
+    apply H_ih_H₂, apply insert_subset_insert, exact image_subset _ h,},
 
-    { apply eqI, },
-    { apply eqE, apply H_ih_H₁ h, apply H_ih_H₂ h, },
+  { apply eqI, },
+  { apply eqE, apply H_ih_H₁ h, apply H_ih_H₂ h, },
 end
 
 /--
   Proof rule for weakening the context of a proof by inserting a single premise.
 -/
-def weak1 {Γ} {φ ψ: formula L} ( H: Γ ⊢ ψ ) :  (φ::Γ) ⊢ ψ := weak Γ H (subset_insert φ Γ)
+def weak1 {Γ} {φ ψ: formula 𝒮} ( H: Γ ⊢ ψ ) :  (φ::Γ) ⊢ ψ := weak Γ H (subset_insert φ Γ)
 
 /--
   Proof rule for weakening the context of a proof from a single premise.
 -/
-def weak_singleton {Γ} (φ) {ψ: formula L} ( H: { φ } ⊢ ψ ) (h: φ ∈ Γ ) :  Γ ⊢ ψ :=
+def weak_singleton {Γ} (φ) {ψ: formula 𝒮} ( H: { φ } ⊢ ψ ) (h: φ ∈ Γ ) :  Γ ⊢ ψ :=
 begin
   apply weak {φ} H,
   assume x xh,
@@ -896,20 +1103,20 @@ begin
 end
 
 -- QoL rules for hypothesis
-def hypI1 {Γ} (φ: formula L)  : (φ :: Γ ) ⊢ φ := hypI (mem_insert φ Γ)
+def hypI1 {Γ} (φ: formula 𝒮)  : (φ :: Γ ) ⊢ φ := hypI (mem_insert φ Γ)
 
-def hypI2 {Γ} (φ ψ: formula L)  : (φ :: ψ :: Γ ) ⊢ ψ := 
+def hypI2 {Γ} (φ ψ: formula 𝒮)  : (φ :: ψ :: Γ ) ⊢ ψ := 
 begin
   apply hypI, right, exact mem_insert ψ Γ,
 end
 /--
   Rule for top introduction.
 -/
-def topI {Γ: set $ formula L} : Γ ⊢ ⊤' := begin apply impI, apply hypI1, end
+def topI {Γ: set $ formula 𝒮} : Γ ⊢ ⊤' := begin apply impI, apply hypI1, end
 
 
 -- rules for implications
-def impE_insert {Γ} {φ ψ: formula L} (H₁ : Γ ⊢ (φ →' ψ )) : φ :: Γ ⊢ ψ  :=
+def impE_insert {Γ} {φ ψ: formula 𝒮} (H₁ : Γ ⊢ (φ →' ψ )) : φ :: Γ ⊢ ψ  :=
 begin
   apply impE φ, 
   apply hypI1, 
@@ -920,15 +1127,15 @@ end
 /--
   Proof rule for reflexivity of implications.
 -/
-def impI_refl {Γ} (φ : formula L) : Γ ⊢ (φ →' φ) := 
+def impI_refl {Γ} (φ : formula 𝒮) : Γ ⊢ (φ →' φ) := 
 begin
     apply impI, apply hypI1,
 end
 
 /--
-  Proof rule for transivity of implications.
+  Proof rule for transitivity of implications.
 -/
-def impI_trans  {Γ} (φ ψ χ : formula L) (H₁: Γ ⊢ (φ →' ψ )) (H₂ : Γ ⊢ (ψ  →' χ )) : Γ ⊢ (φ  →' χ) :=
+def impI_trans  {Γ} (φ ψ χ : formula 𝒮) (H₁: Γ ⊢ (φ →' ψ )) (H₂ : Γ ⊢ (ψ  →' χ )) : Γ ⊢ (φ  →' χ) :=
 begin
   apply impI, 
   apply impE ψ, 
@@ -939,216 +1146,195 @@ end
 /--
   QoL proof rule for universal quantification elimination.
 -/
-def allE' {Γ} (φ) (t: term L) {ψ}  (H : Γ ⊢ (∀'φ)) (h: ψ  = φ[t ⁄ 0]) : Γ ⊢ ψ :=
+def allE' {Γ} (φ) (t: term 𝒮) {ψ}  (H : Γ ⊢ (∀'φ)) (h: ψ  = φ[t ⁄ 0]) : Γ ⊢ ψ :=
 begin subst h, apply allE, assumption, end
 
 /--
   Proof rule for a common case of universal quantification elimination.
 -/
-def allE_var0 {Γ} {φ: formula L}  (H : Γ ⊢ (∀'φ) ↑ 1 ＠ 0) : Γ ⊢ φ  :=
+def allE_var0 {Γ} {φ: formula 𝒮}  (H : Γ ⊢ (∀'φ) ↑ 1 ＠ 0) : Γ ⊢ φ  :=
 begin
-    apply allE' (φ ↑ 1 ＠  1) #0,
-    { exact H, }, 
-    { symmetry, exact subst_var0_lift_by_1 φ 0, } 
+  apply allE' (φ ↑ 1 ＠  1) #0,
+  { exact H, }, 
+  { symmetry, exact subst_var0_lift_by_1 φ 0, } 
 end
 
 
 /--
   Proof rule for equality elimination. _(QoL)_
 -/
-def eqE' {Γ} {ψ}  (s t) (φ : formula L) (H₁ : Γ ⊢ (s =' t)) (H₂ : Γ ⊢ (φ [s ⁄ 0])) (h:  ψ = φ[t ⁄ 0]) : Γ ⊢ ψ :=
+def eqE' {Γ} {ψ}  (s t) (φ : formula 𝒮) (H₁ : Γ ⊢ (s =' t)) (H₂ : Γ ⊢ (φ [s ⁄ 0])) (h:  ψ = φ[t ⁄ 0]) : Γ ⊢ ψ :=
 begin rw h, apply eqE H₁ H₂, end
 
-/--
-  Proof rule for congruence introduction.
--/
-def congrI {Γ} {t s₁ s₂: term L} (H :  Γ ⊢ (s₁ =' s₂)) :  Γ ⊢ ( t[s₁ ⁄ 0] =' t[s₂ ⁄ 0] ):=
+/-- Proof rule for congruence introduction. -/
+def congrI {Γ} {t s₁ s₂: term 𝒮} (H :  Γ ⊢ (s₁ =' s₂)) :  Γ ⊢ ( t[s₁ ⁄ 0] =' t[s₂ ⁄ 0] ):=
 begin
   apply eqE' s₁ s₂ (( (t[s₁⁄ 0] ↑ 1 ＠ 0 )=' t)) H;
   rw [subst, term.subst_for_0_lift_by_1 (term.subst t _ 0) _],
   apply eqI,
 end
-/--
-  Proof rule for congruence introduction. _(QoL)_
--/
-def congrI' {Γ} {t₁ s₁ t₂ s₂ : term L} (t) (H: Γ ⊢ s₁ =' s₂) 
+
+/-- Proof rule for congruence introduction. -/
+def congrI' {Γ} {t₁ s₁ t₂ s₂ : term 𝒮} (t) (H: Γ ⊢ s₁ =' s₂) 
   (h₁: t₁ = t[s₁ ⁄ 0]) (h₂: t₂ = t[s₂ ⁄ 0]) : Γ ⊢ (t₁ =' t₂) := 
 begin rw [h₁, h₂], apply congrI H, end
 
+/-- Proof rule for reflexivity of equality. -/
+def eqI_refl {Γ} (t: term 𝒮): Γ ⊢ (t =' t) := @eqI 𝒮 Γ t
 
-/--
-  Proof rule for reflexivity of equality.
--/
-def eqI_refl {Γ} (t: term L): Γ ⊢ (t =' t) := @eqI L Γ t
-/--
-  Proof rule for symmetry of equality.
--/
-def eqI_symm {Γ} (s t : term L) (H : Γ ⊢ (s =' t)) : Γ ⊢ (t =' s) :=
+/-- Proof rule for symmetry of equality. -/
+def eqI_symm {Γ} (s t : term 𝒮) (H : Γ ⊢ (s =' t)) : Γ ⊢ (t =' s) :=
 begin
-    apply eqE' s t (#0 =' (s ↑ 1 ＠ 0)) H;
-    rw [subst, term.subst_var0, term.subst_for_0_lift_by_1],
-    apply eqI, 
+  apply eqE' s t (#0 =' (s ↑ 1 ＠ 0)) H;
+  rw [subst, term.subst_var0, term.subst_for_0_lift_by_1],
+  apply eqI, 
 end
-/--
-  Proof rule for transitivity of equality.
--/
-def eqI_trans {Γ} ( s t u : term L) (H₁ : Γ ⊢ (s =' t) ) (H₂ : Γ ⊢ (t =' u)) : proof Γ ( s =' u) :=
+/-- Proof rule for transitivity of equality. -/
+def eqI_trans {Γ} ( s t u : term 𝒮) (H₁ : Γ ⊢ (s =' t) ) (H₂ : Γ ⊢ (t =' u)) : proof Γ ( s =' u) :=
 begin
   apply eqE' t u ((s ↑ 1 ＠ 0) =' #0) H₂;
   rw[subst, term.subst_for_0_lift_by_1, term.subst_var0], 
   assumption,
 end
 
+/- biconditionals -/
 
-/--
-  Proof rule for introducing a biconditional.
--/
-def iffI {Γ} {φ ψ : formula L} (H₁ : Γ ⊢ φ →' ψ) (H₂ : Γ ⊢ ψ →' φ)  : Γ ⊢ (φ  ↔' ψ) :=
+/-- Proof rule for introducing a biconditional. -/
+def iffI {Γ} {φ ψ : formula 𝒮} (H₁ : Γ ⊢ φ →' ψ) (H₂ : Γ ⊢ ψ →' φ)  : Γ ⊢ (φ  ↔' ψ) :=
 begin apply andI; assumption, end
 
-def iffE_r {Γ} {φ ψ : formula L} (H : Γ ⊢ φ ↔' ψ)  : (Γ ⊢ φ →' ψ) := andE₁ _ H
+def iffE_r {Γ} {φ ψ : formula 𝒮} (H : Γ ⊢ φ ↔' ψ)  : (Γ ⊢ φ →' ψ) := andE₁ _ H
 
-def iffE_l {Γ} {φ ψ : formula L} (H : Γ ⊢ φ ↔' ψ)  : (Γ ⊢ ψ →' φ) := andE₂ _ H
+def iffE_l {Γ} {φ ψ : formula 𝒮} (H : Γ ⊢ φ ↔' ψ)  : (Γ ⊢ ψ →' φ) := andE₂ _ H
 
 /--
   Proof rule for eliminating the right part of a biconditional.
 -/
-def iffE₁ {Γ} {φ: formula L} (ψ : formula L) (H₁ : Γ ⊢ ψ) (H₂ : Γ ⊢ φ ↔' ψ)  : Γ ⊢ φ :=
+def iffE₁ {Γ} {φ: formula 𝒮} (ψ : formula 𝒮) (H₁ : Γ ⊢ ψ) (H₂ : Γ ⊢ φ ↔' ψ)  : Γ ⊢ φ :=
 begin
   apply impE ψ,
   { exact H₁, },
   { apply andE₂, exact H₂, },
 end
 
-/--
-  Proof rule for eliminating the left part of a biconditional.
--/
-def iffE₂ {Γ} (φ) {ψ : formula L} (H₁ : Γ ⊢ φ) (H₂ : Γ ⊢ φ ↔' ψ)  : (Γ ⊢  ψ) :=
+/-- Proof rule for eliminating the left part of a biconditional. -/
+def iffE₂ {Γ} (φ) {ψ : formula 𝒮} (H₁ : Γ ⊢ φ) (H₂ : Γ ⊢ φ ↔' ψ)  : (Γ ⊢  ψ) :=
 begin
   apply impE φ,
   { exact H₁, },
   { apply andE₁, exact H₂, },
 end
 
-/--
-  Proof rule for reflexivity of biconditionals.
--/
-def iffI_refl {Γ} (φ : formula L) : Γ ⊢ (φ ↔' φ) := begin apply iffI; apply impI_refl,end
-/--
-  Proof rule for transitivity of biconditionals.
--/
-def iffI_trans {Γ} {φ} (ψ: formula L) {χ}  (H₁: Γ ⊢ (φ ↔' ψ)) (H₂ : Γ ⊢ (ψ ↔' χ)) : Γ ⊢ (φ ↔' χ) :=
+/-- Proof rule for reflexivity of biconditionals.-/
+def iffI_refl {Γ} (φ : formula 𝒮) : Γ ⊢ (φ ↔' φ) := begin apply iffI; apply impI_refl,end
+
+/-- Proof rule for transitivity of biconditionals. -/
+def iffI_trans {Γ} {φ} (ψ: formula 𝒮) {χ}  (H₁: Γ ⊢ (φ ↔' ψ)) (H₂ : Γ ⊢ (ψ ↔' χ)) : Γ ⊢ (φ ↔' χ) :=
 begin
     apply andI;
     apply impI_trans _ ψ _,
     apply andE₁ _ H₁, apply andE₁ _ H₂,
     apply andE₂ _ H₂, apply andE₂ _ H₁,
 end
-/--
-  Proof rule for symmetry of biconditionals.
--/
-def iffI_symm {Γ} {φ ψ: formula L}  (H: Γ ⊢ (φ ↔' ψ)) : Γ ⊢ (ψ ↔' φ) := 
+
+/-- Proof rule for symmetry of biconditionals. -/
+def iffI_symm {Γ} {φ ψ: formula 𝒮}  (H: Γ ⊢ (φ ↔' ψ)) : Γ ⊢ (ψ ↔' φ) := 
 begin apply iffI, apply andE₂, exact H, apply andE₁, exact H, end
 
--- rules for lifting and substitutions
-/--
-  Proof rule for substiuting a term for free variable .
--/
-def substI {Γ} {φ : formula L} (t k) (H: Γ ⊢ φ ) : (λ ϕ, ϕ[t ⁄ k])'' Γ ⊢ φ[t ⁄ k] :=
+
+/-- Proof rule for substiuting a term for free variable. -/
+def substI {Γ} {φ : formula 𝒮} (t k) (H: Γ ⊢ φ ) : (λ ϕ, ϕ[t ⁄ k])'' Γ ⊢ φ[t ⁄ k] :=
 begin
-    induction H generalizing k,
-    { apply hypI, exact mem_image_of_mem (λ (ϕ : preformula L 0), ϕ [t ⁄ k]) H_h, },
-    { apply botE, apply H_ih, },
+  induction H generalizing k,
+  { apply hypI, exact mem_image_of_mem (λ (ϕ : preformula 𝒮 0), ϕ [t ⁄ k]) H_h, },
+  { apply botE, apply H_ih, },
 
-    { apply impI, rw ← (@image_insert_eq _ _ (λ (x : preformula L 0), x[t ⁄ k])), exact H_ih k, },
-    { apply impE (H_φ [t ⁄ k]), exact H_ih_H₁ k, exact H_ih_H₂ k, },
+  { apply impI, rw ← (@image_insert_eq _ _ (λ (x : preformula 𝒮 0), x[t ⁄ k])), exact H_ih k, },
+  { apply impE (H_φ [t ⁄ k]), exact H_ih_H₁ k, exact H_ih_H₂ k, },
 
-    { apply andI, exact H_ih_H₁ k, exact H_ih_H₂ k, },
-    { apply andE₁, exact H_ih k, },
-    { apply andE₂, exact H_ih k, },
+  { apply andI, exact H_ih_H₁ k, exact H_ih_H₂ k, },
+  { apply andE₁, exact H_ih k, },
+  { apply andE₂, exact H_ih k, },
 
-    { apply orI₁, exact H_ih k, },
-    { apply orI₂, exact H_ih k, },
-    { apply orE (H_φ [t ⁄ k]) (H_ψ [t ⁄ k]), 
-      apply H_ih_H k, 
-      have H₁:= H_ih_H₁ k, rw image_insert_eq at H₁, exact H₁,
-      have H₂:= H_ih_H₂ k, rw image_insert_eq at H₂, exact H₂, },
+  { apply orI₁, exact H_ih k, },
+  { apply orI₂, exact H_ih k, },
+  { apply orE (H_φ [t ⁄ k]) (H_ψ [t ⁄ k]), 
+    apply H_ih_H k, 
+    have H₁:= H_ih_H₁ k, rw image_insert_eq at H₁, exact H₁,
+    have H₂:= H_ih_H₂ k, rw image_insert_eq at H₂, exact H₂, },
 
-    { apply allI, rw [image_image, lambda_lift_subst_formula(k.zero_le)], 
-      have H := H_ih (k+1), rw image_image at H, exact H, },
-    { apply allE' _ (H_t[t ⁄ k]) (H_ih k), apply subst_subst, exact (k.zero_le), },
+  { apply allI, rw [image_image, lambda_lift_subst_formula(k.zero_le)], 
+    have H := H_ih (k+1), rw[image_image] at H, exact H, },
+  { apply allE' _ (H_t[t ⁄ k]) (H_ih k), apply subst_subst, exact (k.zero_le), },
+
+  { apply exI (H_t [t⁄ k]), 
+      have h:= subst_subst H_φ H_t t (k.zero_le), 
+      rw nat.sub_zero at h, rw ←h, exact H_ih k,},
+  { apply exE (H_φ [t⁄(k+1)]), apply H_ih_H₁ k, rw lift_subst H_ψ t 1 0 k (k.zero_le),
+      have h:= H_ih_H₂ (k+1),
+      rw [image_insert_eq, image_image, ←lambda_lift_subst_formula(k.zero_le)] at h,
+      rw [image_image], exact h, },
   
-    { apply exI (H_t [t⁄ k]), 
-        have h:= subst_subst H_φ H_t t (k.zero_le), 
-        rw nat.sub_zero at h, rw ←h, exact H_ih k,},
-    { apply exE (H_φ [t⁄(k+1)]), apply H_ih_H₁ k, rw lift_subst H_ψ t 1 0 k (k.zero_le),
-        have h:= H_ih_H₂ (k+1),
-        rw [image_insert_eq, image_image, ←lambda_lift_subst_formula(k.zero_le)] at h,
-        rw [image_image], exact h, },
-    
-    { apply eqI_refl, },
-    { apply eqE', apply H_ih_H₁ k,
-      have h:= H_ih_H₂ k, rwa [subst_subst H_φ H_s t (k.zero_le), nat.sub_zero] at h, 
-      exact subst_subst H_φ H_t t (k.zero_le), }
+  { apply eqI_refl, },
+  { apply eqE', apply H_ih_H₁ k,
+    have h:= H_ih_H₂ k, rwa [subst_subst H_φ H_s t (k.zero_le), nat.sub_zero] at h, 
+    exact subst_subst H_φ H_t t (k.zero_le), }
 end
 
-/--
-  Proof rule for introducing `m` fresh variables at index `i` to a proof.
--/
-def liftI {Γ} {φ  : formula L} (m i : ℕ) (H: Γ ⊢ φ ) : (λ (ϕ :formula L), ϕ ↑ m ＠  i ) '' Γ ⊢ (φ ↑ m ＠  i) :=
+/-- Proof rule for introducing `m` fresh variables at index `i` to a proof. -/
+def liftI {Γ} {φ : formula 𝒮} (m i : ℕ) (H: Γ ⊢ φ) : (λ (ϕ :formula 𝒮), ϕ ↑ m ＠  i ) '' Γ ⊢ (φ ↑ m ＠  i) :=
 begin
-    induction H generalizing i,
-    { apply hypI, exact mem_image_of_mem (λ (ϕ : preformula L 0),  ϕ ↑ m ＠  i) H_h, },
-    { apply botE, exact H_ih i, },
+  induction H generalizing i,
+  { apply hypI, exact mem_image_of_mem (λ (ϕ : preformula 𝒮 0),  ϕ ↑ m ＠  i) H_h, },
+  { apply botE, exact H_ih i, },
 
-    { apply impI, have:= H_ih i, rwa image_insert_eq at this, },
-    { apply impE (H_φ ↑ m ＠  i) , exact H_ih_H₁ i, exact H_ih_H₂ i,},
+  { apply impI, have:= H_ih i, rwa image_insert_eq at this, },
+  { apply impE (H_φ ↑ m ＠  i) , exact H_ih_H₁ i, exact H_ih_H₂ i,},
 
-    { apply andI, apply H_ih_H₁ i, apply H_ih_H₂ i, },
-    { apply andE₁, apply H_ih i, },
-    { apply andE₂, apply H_ih i, },
+  { apply andI, apply H_ih_H₁ i, apply H_ih_H₂ i, },
+  { apply andE₁, apply H_ih i, },
+  { apply andE₂, apply H_ih i, },
 
-    { apply orI₁, apply H_ih i, },
-    { apply orI₂, apply H_ih i, },
-    { apply orE, apply H_ih_H i,
-      have H₁:= H_ih_H₁ i, rw image_insert_eq at H₁, exact H₁,
-      have H₂:= H_ih_H₂ i, rw image_insert_eq at H₂, exact H₂, },
-    
-    { apply allI, rw[image_image, lambda_lift_lift _ _ (i.zero_le)],
-      have h:= H_ih (i+1), rw image_image at h, exact h, },
-    { apply allE' _ (H_t ↑ m ＠ i) (H_ih i), 
-      have h := eq.symm (subst_lift_in_lift H_φ H_t m i 0), exact h,},
+  { apply orI₁, apply H_ih i, },
+  { apply orI₂, apply H_ih i, },
+  { apply orE, apply H_ih_H i,
+    have H₁ := H_ih_H₁ i, rw image_insert_eq at H₁, exact H₁,
+    have H₂ := H_ih_H₂ i, rw image_insert_eq at H₂, exact H₂, },
+  
+  { apply allI, rw[image_image, lambda_lift_lift _ _ (i.zero_le)],
+    have h:= H_ih (i+1), rw[image_image] at h, exact h, },
+  { apply allE' _ (H_t ↑ m ＠ i) (H_ih i), 
+    have h := eq.symm (subst_lift_in_lift H_φ H_t m i 0), exact h,},
 
-    { apply exI (H_t ↑ m ＠ i), 
-      rw subst0_lift_by_lift H_φ, 
-      exact H_ih i,  },
-    { apply exE (H_φ ↑ m ＠ (i+1)), apply H_ih_H₁ i, 
-      rw[image_image, lift_lift H_ψ m 1 (i.zero_le), lambda_lift_lift _ _ (i.zero_le)],
-      have h := H_ih_H₂ (i+1), rw[image_insert_eq, image_image] at h, exact h, },
-    
-    { apply eqI_refl, },
-    { apply eqE' _ _ _ (H_ih_H₁ i),
-      have h₁:= symm (subst0_lift_by_lift H_φ),
-      have h₂ := H_ih_H₂ i, rw h₁ at h₂, exact h₂,
-      exact symm ( subst0_lift_by_lift _ ), },
+  { apply exI (H_t ↑ m ＠ i), 
+    rw subst0_lift_by_lift H_φ, 
+    exact H_ih i,  },
+  { apply exE (H_φ ↑ m ＠ (i+1)), apply H_ih_H₁ i, 
+    rw[image_image, lift_lift H_ψ m 1 (i.zero_le), lambda_lift_lift _ _ (i.zero_le)],
+    have h := H_ih_H₂ (i+1), rw[image_insert_eq, image_image] at h, exact h, },
+  
+  { apply eqI_refl, },
+  { apply eqE' _ _ _ (H_ih_H₁ i),
+    have h₁:= symm (subst0_lift_by_lift H_φ),
+    have h₂ := H_ih_H₂ i, rw h₁ at h₂, exact h₂,
+    exact symm ( subst0_lift_by_lift _ ), },
 end
-
 
 -- rules for dealing with universal closures
-def allsI {Γ} {φ: formula L}  (n) (H: (λ ϕ , ϕ ↑ n ＠  0) '' Γ ⊢ φ) :  Γ ⊢ alls n φ  :=
+def allsI {Γ} {φ: formula 𝒮}  (n) (H: (λ ϕ , ϕ ↑ n ＠  0) '' Γ ⊢ φ) :  Γ ⊢ alls n φ  :=
 begin
   induction n generalizing φ Γ,
   { simp [lift_by_0] at H, assumption,},
   { rw[alls], 
     apply allI,
-    have h : (λ (ϕ : preformula L 0), ϕ ↑ n_n.succ ＠ 0) 
-      = (λ (ϕ : preformula L 0), ϕ ↑ n_n ＠ 0) ∘ (λ (ϕ : preformula L 0), ϕ ↑ 1＠ 0),
+    have h : (λ (ϕ : preformula 𝒮 0), ϕ ↑ n_n.succ ＠ 0) 
+      = (λ (ϕ : preformula 𝒮 0), ϕ ↑ n_n ＠ 0) ∘ (λ (ϕ : preformula 𝒮 0), ϕ ↑ 1＠ 0),
     begin funext, dsimp, rw lift_at_lift_merge, rw add_comm 1 n_n, end,
     rw [h, image_comp] at H,
     exact n_ih H, },
 end
 
-def allsE  {Γ} {φ: formula L}  (n i) (H :  Γ ⊢ (alls n φ)) :  Γ ⊢ substs n i 0 φ :=
+def allsE  {Γ} {φ: formula 𝒮}  (n i) (H :  Γ ⊢ (alls n φ)) :  Γ ⊢ substs n i 0 φ :=
 begin
   induction n generalizing φ i,
   { exact H,},
@@ -1159,14 +1345,14 @@ begin
     exact n_ih (i+1) H, },
 end
 
-def allsE' {Γ} (n) {φ  : formula L} (H : Γ ⊢ (alls n φ)) : (λ ϕ , ϕ ↑ n ＠  0) '' Γ ⊢ φ  :=
+def allsE' {Γ} (n) {φ  : formula 𝒮} (H : Γ ⊢ (alls n φ)) : (λ ϕ , ϕ ↑ n ＠  0) '' Γ ⊢ φ  :=
 begin
   induction n generalizing φ Γ,
-  { have h :  (λ (ϕ: formula L) , ϕ ↑ 0 ＠  0) = id, from begin funext, rw lift_by_0, refl, end,
+  { have h :  (λ (ϕ: formula 𝒮) , ϕ ↑ 0 ＠  0) = id, from begin funext, rw lift_by_0, refl, end,
     rw [h, image_id] at *, 
     rwa alls at H, },
-  { have h: (λ (ϕ : preformula L 0), ϕ ↑ n_n.succ ＠ 0) 
-          = (λ (ϕ : preformula L 0), ϕ ↑ 1 ＠ 0) ∘ (λ (ϕ : preformula L 0), ϕ ↑ n_n ＠ 0),
+  { have h: (λ (ϕ : preformula 𝒮 0), ϕ ↑ n_n.succ ＠ 0) 
+          = (λ (ϕ : preformula 𝒮 0), ϕ ↑ 1 ＠ 0) ∘ (λ (ϕ : preformula 𝒮 0), ϕ ↑ n_n ＠ 0),
     begin funext, dsimp, rw lift_at_lift_merge, end,
     rw [alls_succ] at H,
     apply allE_var0,
@@ -1175,7 +1361,7 @@ begin
     exact n_ih H, },
 end
 
-def modus_tollens {Γ} {φ} (ψ: formula L) (H₁: Γ ⊢ (φ →' ψ)) (H₂: Γ ⊢ ¬'ψ) : Γ ⊢ ¬'φ  :=
+def modus_tollens {Γ} {φ} (ψ: formula 𝒮) (H₁: Γ ⊢ (φ →' ψ)) (H₂: Γ ⊢ ¬'ψ) : Γ ⊢ ¬'φ  :=
 begin
   apply impI,
   apply impE ψ,
@@ -1188,10 +1374,8 @@ end proof
 
 export proof
 
-/--
-  Formal proof that there always exists an object of discourse,
--/
-def let_there_be_light : (∅ : set $ formula L) ⊢ ∃'(#0 =' #0) :=
+/-- Formal proof that there always exists an object of discourse. -/
+def let_there_be_light : (∅ : set $ formula 𝒮) ⊢ ∃'(#0 =' #0) :=
 begin
   apply exI #0,
   apply eqI,
@@ -1203,7 +1387,7 @@ end
    Therefore, Socrates is mortal." .   
 -/
 
-example {Γ:set $ formula L}{φ ψ χ}  (H₁: Γ ⊢ ∀'(φ →' ψ))  (H₂: Γ ⊢ ∀'(ψ →' χ)) : Γ ⊢ ∀' (φ →' χ) :=
+example {Γ:set $ formula 𝒮}{φ ψ χ}  (H₁: Γ ⊢ ∀'(φ →' ψ))  (H₂: Γ ⊢ ∀'(ψ →' χ)) : Γ ⊢ ∀' (φ →' χ) :=
 begin
   apply allI,
   apply impI,
@@ -1222,7 +1406,7 @@ begin
     rw subst_var0_lift_by_1, },
 end
 
-example {Γ:set $ formula L}{φ ψ χ}  (H₁: Γ ⊢ ∀'(φ →' ψ) )  (H₂: Γ ⊢ ∀'(ψ →' χ)) : Γ ⊢ ∀' (φ →' χ) :=
+example {Γ:set $ formula 𝒮}{φ ψ χ}  (H₁: Γ ⊢ ∀'(φ →' ψ) )  (H₂: Γ ⊢ ∀'(ψ →' χ)) : Γ ⊢ ∀' (φ →' χ) :=
 begin
   apply allI,
   apply impI,
@@ -1238,4 +1422,7 @@ begin
     rw subst_var0_lift_by_1,
     assumption, },
 end
+
+end proof_terms
+
 end fol
